Corrected sim-star and sim-plus for eqauls (with Gordon), extend, and inject. Propagating the correctsions through compiler proof partly done - currently stuck do to repeated Coq error message
Anomaly: Cannot take the successor of a non variable universe:
(maybe a bugged tactic).
Please report.

in places where congruence is called. Will investigate why universes issue arises all of a sudden tomorrow....

veric/CminorgenproofSIM.v
@@ -22,9 +22,6 @@ Proof. intros.  unfold mem_forward in FWD. unfold Mem.valid_block in FWD.
    specialize (FWD (Mem.nextblock m - 1)). omega.
 Qed.
 
-Lemma inject_separated_same_meminj: forall j m m', Events.inject_separated j j m m'.
-  Proof. intros j m m' b; intros. congruence. Qed.
-
 Lemma allocvars_blocks_valid: forall vars E m e m1,
  alloc_variables E m vars e m1 -> 
  forall b, Mem.valid_block m b -> Mem.valid_block m1 b.
@@ -62,11 +59,11 @@ Let ge : Csharpminor.genv := Genv.globalenv prog.
 Let gce : compilenv := build_global_compilenv prog.
 Let tge: genv := Genv.globalenv tprog.
 
-Let core_data := unit.
+Let core_data := CSharpMin_core.
 
 Inductive match_cores: core_data -> meminj -> CSharpMin_core -> mem -> CMin_core -> mem -> Prop :=
   | MC_states:
-      forall fn s k e le m tfn ts tk sp te tm cenv xenv j lo hi cs sz
+      forall d fn s k e le m tfn ts tk sp te tm cenv xenv j lo hi cs sz
       (TRF: transl_funbody cenv sz fn = OK tfn)
       (TR: transl_stmt fn.(fn_return) cenv xenv s = OK ts)
       (MINJ: Mem.inject j m tm)
@@ -74,10 +71,10 @@ Inductive match_cores: core_data -> meminj -> CSharpMin_core -> mem -> CMin_core
                (Frame cenv tfn e le te sp lo hi :: cs)
                (Mem.nextblock m) (Mem.nextblock tm))
       (MK: match_cont k tk fn.(fn_return) cenv xenv cs),
-      match_cores tt j (CSharpMin_State fn s k e le) m
+      match_cores d j (CSharpMin_State fn s k e le) m
                    (CMin_State tfn ts tk (Vptr sp Int.zero) te) tm
   | MC_state_seq:
-      forall fn s1 s2 k e le m tfn ts1 tk sp te tm cenv xenv j lo hi cs sz
+      forall d fn s1 s2 k e le m tfn ts1 tk sp te tm cenv xenv j lo hi cs sz
       (TRF: transl_funbody cenv sz fn = OK tfn)
       (TR: transl_stmt fn.(fn_return) cenv xenv s1 = OK ts1)
       (MINJ: Mem.inject j m tm)
@@ -85,10 +82,10 @@ Inductive match_cores: core_data -> meminj -> CSharpMin_core -> mem -> CMin_core
                (Frame cenv tfn e le te sp lo hi :: cs)
                (Mem.nextblock m) (Mem.nextblock tm))
       (MK: match_cont (Csharpminor.Kseq s2 k) tk fn.(fn_return) cenv xenv cs),
-      match_cores tt j (CSharpMin_State fn (Csharpminor.Sseq s1 s2) k e le) m
+      match_cores d j (CSharpMin_State fn (Csharpminor.Sseq s1 s2) k e le) m
                    (CMin_State tfn ts1 tk (Vptr sp Int.zero) te) tm
   | MC_callstate:
-      forall fd args k m tfd targs tk tm j cs cenv
+      forall d fd args k m tfd targs tk tm j cs cenv
       (TR: transl_fundef gce fd = OK tfd)
       (MINJ: Mem.inject j m tm)
       (MCS: match_callstack prog j m tm cs (Mem.nextblock m) (Mem.nextblock tm))
@@ -104,18 +101,30 @@ Inductive match_cores: core_data -> meminj -> CSharpMin_core -> mem -> CMin_core
      (ARGSTYP: Forall2 Val.has_type args (Csharpminor.funsig fd).(sig_args))
      (TARGSTYP: Forall2 Val.has_type targs (Csharpminor.funsig fd).(sig_args)),
  
-      match_cores tt j (CSharpMin_Callstate fd args k) m
+      match_cores d j (CSharpMin_Callstate fd args k) m
                    (CMin_Callstate tfd targs tk) tm
   | MC_returnstate:
-      forall v k m tv tk tm j cs ty cenv
+      forall d v k m tv tk tm j cs ty cenv
       (MINJ: Mem.inject j m tm)
       (MCS: match_callstack prog j m tm cs (Mem.nextblock m) (Mem.nextblock tm))
       (MK: match_cont k tk ty cenv nil cs)
       (RESINJ: val_inject j v tv),
-      match_cores tt j (CSharpMin_Returnstate v k) m
+      match_cores d j (CSharpMin_Returnstate v k) m
                    (CMin_Returnstate tv tk) tm.
 
-Lemma init_cores: forall v1 v2 vals1 (c1 : CSharpMin_core) m1 j vals2 m2 
+Lemma init_cores: forall (v1 v2 : val) (sig : signature) entrypoints
+(EP: In (v1, v2, sig) entrypoints)
+  (vals1 : list val) (c1 : core_data) (m1 : mem) (j : meminj)
+  (vals2 : list val) (m2 : mem)
+ (CSM_Ini : make_initial_core CSharpMin_CompcertCoreSem ge v1 vals1 = Some c1)
+ (Inj : Mem.inject j m1 m2)
+ (VI: Forall2 (val_inject j) vals1 vals2)
+ (HT: Forall2 Val.has_type vals2 (sig_args sig)),
+exists c2 : CMin_core,
+  make_initial_core CMin_CompcertCoreSem tge v2 vals2 = Some c2 /\
+  match_cores c1 j c1 m1 c2 m2. 
+(*
+v1 v2 vals1 (c1 : CSharpMin_core) m1 j vals2 m2 
       sig
       (CSM_Ini : make_initial_core CSharpMin_CompcertCoreSem ge v1 vals1 = Some c1)
       (Inj : Mem.inject j m1 m2)
@@ -124,7 +133,7 @@ Lemma init_cores: forall v1 v2 vals1 (c1 : CSharpMin_core) m1 j vals2 m2
 exists cd : core_data,
   exists c2 : CMin_core,
     make_initial_core CMin_CompcertCoreSem tge v2 vals2 = Some c2 /\
-    match_cores cd j c1 m1 c2 m2.
+    match_cores cd j c1 m1 c2 m2.*)
 Proof.
   intros. inv CSM_Ini.
   unfold  CSharpMin_make_initial_core in H0.
@@ -136,7 +145,8 @@ Proof.
                               destruct t; try inv H0.
   apply eq_sym in Heqzz.
   destruct (function_ptr_translated _ _ TRANSL _ _ Heqzz) as [tf [FIND TR]].  
-  exists tt. eexists.
+    (*unfold core_data. exists (CSharpMin_Callstate f nil Csharpminor.Kstop).*)
+   eexists.
   split.
   (*make_initial_core*)
       simpl. unfold CMin_make_initial_core.
@@ -147,9 +157,12 @@ Proof.
         rewrite (sig_preserved _ _ _ TR). rewrite <- Heqfs. reflexivity.
   (*match_cores*)
   eapply MC_callstate with (j := j) (cs := @nil frame); try eassumption.
-      Focus 2. econstructor.
-      Focus 2. econstructor.
-      Focus 2. econstructor.
+     admit. (*some error here wrt initial mems*)
+      econstructor.
+      econstructor.
+      econstructor.
+      rewrite <- Heqfs. simpl. constructor.
+      rewrite <- Heqfs. simpl. constructor.
 (*   
      destruct Inj. clear HT VI vals1 vals2 Heqz Heqzz Heqfs FIND TR f tf. destruct mi_inj.
      apply mcs_nil with (Mem.nextblock m1). 
@@ -168,40 +181,39 @@ safely_halted CSharpMin_CompcertCoreSem ge c1 = Some v1 ->
 safely_halted CMin_CompcertCoreSem tge c2 = Some v1 /\ Mem.inject j m1 m2.
 Proof.
   intros.
-  inv H; simpl in *; try congruence.
-     inv RESINJ; simpl in *; trivial; try congruence.
-         inv MK; try congruence.
-           split; assumption.
+  inv H; simpl in *; inv H0.
+     inv RESINJ; simpl in *; trivial; inv H1.
+         inv MK; inv H0.
+           split; trivial.
 Qed.
 
 Lemma MC_at_external: forall (cd : core_data) (j : meminj) (st1 : CSharpMin_core) (m1 : mem)
   (st2 : CMin_core) (m2 : mem) (e : external_function) (vals1 : list val) sig,
-match_cores cd j st1 m1 st2 m2 ->
+(cd = st1 /\ match_cores cd j st1 m1 st2 m2) ->
 at_external CSharpMin_CompcertCoreSem st1 = Some (e, sig, vals1) ->
 Mem.inject j m1 m2 /\
 Events.meminj_preserves_globals ge j /\
 (exists vals2 : list val,
    Forall2 (val_inject j) vals1 vals2 /\
-   Forall2 Val.has_type vals2 (sig_args (ef_sig e)) /\
+   Forall2 Val.has_type vals2 (sig_args sig) /\
    at_external CMin_CompcertCoreSem st2 = Some (e, sig, vals2)).
 Proof.
-  intros.
-  inv H; simpl in *; try congruence.
+  intros. destruct H; subst.
+  inv H1; simpl in *; inv H0.
   split; trivial.
   split. destruct (match_callstack_match_globalenvs _ _ _ _ _ _ _ MCS) as [hi Hhi].
               eapply inj_preserves_globals; eassumption.
-  destruct fd; try congruence. inv H0.
+  destruct fd; inv H1.
   exists targs.
   split. eapply val_list_inject_forall_inject; eassumption.
   inv TR.
   split; trivial.
 Qed.
 
-Lemma MC_after_external:forall (cd : core_data) (j j' : meminj) (st1 : CSharpMin_core)
-  (st2 : CMin_core) (m1 : mem) (e : external_function) (vals1 : list val) sig
-  (ret1 : val) (m1' m2 m2' : mem) (ret2 : val),
-Mem.inject j m1 m2 ->
-match_cores cd j st1 m1 st2 m2 ->
+Lemma MC_after_external:forall (d : core_data) (j j' : meminj) (st1 : core_data) (st2 : CMin_core)
+  (m1 : mem) (e : external_function) (vals1 : list val) (ret1 : val)
+  (m1' m2 m2' : mem) (ret2 : val) (sig : signature),
+d = st1 /\ match_cores d j st1 m1 st2 m2 ->
 at_external CSharpMin_CompcertCoreSem st1 = Some (e, sig, vals1) ->
 Events.meminj_preserves_globals ge j ->
 inject_incr j j' ->
@@ -212,30 +224,32 @@ mem_forward m1 m1' ->
 Events.mem_unchanged_on (Events.loc_unmapped j) m1 m1' ->
 mem_forward m2 m2' ->
 Events.mem_unchanged_on (Events.loc_out_of_reach j m1) m2 m2' ->
-Val.has_type ret2 (proj_sig_res (ef_sig e)) ->
-exists cd' : core_data,
-  exists st1' : CSharpMin_core,
-    exists st2' : CMin_core,
+Val.has_type ret2 (proj_sig_res sig) ->
+exists st1' : core_data,
+  exists st2' : CMin_core,
+    exists d' : core_data,
       after_external CSharpMin_CompcertCoreSem (Some ret1) st1 = Some st1' /\
       after_external CMin_CompcertCoreSem (Some ret2) st2 = Some st2' /\
-      match_cores cd' j' st1' m1' st2' m2'.
+      d' = st1' /\ match_cores d' j' st1' m1' st2' m2'. 
 Proof. intros.
-  destruct (MC_at_external _ _ _ _ _ _ _ _ _ H0 H1) as [_ [_ [vals2 [ValsInj [vals2Typ AtExt2]]]]].
-  inv H0; simpl in *; try congruence.
-  destruct fd; try congruence. inv H1.
-  destruct tfd; try congruence. inv AtExt2.
-  exists tt. eexists. eexists.
+  destruct (MC_at_external _ _ _ _ _ _ _ _ _ H H0) as [_ [_ [vals2 [ValsInj [vals2Typ AtExt2]]]]].
+  destruct H as [X MC]; subst.
+  inv MC; simpl in *; inv H0.
+  destruct fd; inv H11.
+  destruct tfd; inv AtExt2.
+  exists (CSharpMin_Returnstate ret1 k). eexists. eexists.
+    split. reflexivity.
     split. reflexivity.
     split. reflexivity.
   simpl in *.
   econstructor; try eassumption.
-  clear TR H12.
+  clear TR H11.
   destruct k; simpl in *; try contradiction. (*cases k = Kseq and k=Kblock eliminated*)
   (*k=Kstop*) 
       inv MK; simpl in *.   
       apply match_callstack_incr_bound with (Mem.nextblock m1) (Mem.nextblock m2).
       eapply match_callstack_external_call; eauto.
-          intros. eapply H7; eauto.
+          intros. eapply H6; eauto.
           omega.
           omega.
          eapply mem_forward_nextblock; assumption.
@@ -244,25 +258,16 @@ Proof. intros.
       inv MK; simpl in *.   
       apply match_callstack_incr_bound with (Mem.nextblock m1) (Mem.nextblock m2).
       eapply match_callstack_external_call; eauto.
-          intros. eapply H7; eauto.
+          intros. eapply H6; eauto.
           omega.
           omega.
          eapply mem_forward_nextblock; assumption.
          eapply mem_forward_nextblock; assumption.
 Qed.
 
-Parameter MC_order :  core_data -> core_data -> Prop. 
-Parameter MC_wellfounded: well_founded MC_order.
-(*Definition MC_measure (q:CSharpMin_core): nat :=
-  match q with
-  | CSharpMin_State fn s k e le => seq_left_depth s
-  | _ => O
-  end.*)
-Parameter MC_measure: CSharpMin_core-> nat.
-
-Lemma MC_MSI: forall j
+Lemma MC_MSI: forall d j
        q m q' m',
-      match_cores tt j q m q' m' -> 
+      match_cores d j q m q' m' -> 
       match_statesInj prog j  (ToState q m) (Cminor_CompcertSemantics.ToState q' m').
   Proof. intros.
     inv H; simpl in *.
@@ -272,9 +277,9 @@ Lemma MC_MSI: forall j
      eapply matchInj_returnstate; try eassumption.
 Qed.  
 
-Lemma MSI_MC: forall j q m q' m',
+Lemma MSI_MC: forall j q m q' m' d,
       match_statesInj prog j (ToState q m) (Cminor_CompcertSemantics.ToState q' m') ->
-      match_cores tt j q m q' m'.
+      match_cores d j q m q' m'.
   Proof. intros.
     inv H; simpl in *.
      destruct q; simpl in *; inv H2.
@@ -304,18 +309,28 @@ Proof.
   apply prop_ext. split; intros; inv H.
 Qed.
 
+Parameter MC_order :  core_data -> core_data -> Prop. 
+Parameter MC_wellfounded: well_founded MC_order.
+Definition MC_measure (q:CSharpMin_core): nat :=
+  match q with
+  | CSharpMin_State fn s k e lenv => seq_left_depth s
+  | _ => O
+  end.
+(*Parameter MC_measure: CSharpMin_core-> nat.*)
+
 Lemma MS_step_case_SkipSeq:
-forall cenv sz f tfn j m tm  e le te sp lo hi cs s k tk xenv
+forall cenv sz f tfn j m tm  e lenv te sp lo hi cs s k tk xenv
 (TRF : transl_funbody cenv sz f = OK tfn)
 (MINJ : Mem.inject j m tm)
 (MK : match_cont (Csharpminor.Kseq s k) tk (fn_return f) cenv xenv cs)
-(MCS : match_callstack prog j m tm (Frame cenv tfn e le te sp lo hi :: cs)
+(MCS : match_callstack prog j m tm (Frame cenv tfn e lenv te sp lo hi :: cs)
         (Mem.nextblock m) (Mem.nextblock tm)),
 exists c2' : CMin_core,
   exists m2' : mem,
         corestep_plus CMin_core_sem tge (CMin_State tfn Sskip tk (Vptr sp Int.zero) te) tm c2' m2' /\
-   exists c' : CSharpMin_core,
-        inj_match_states_star unit match_cores MC_measure (tt,c') j (CSharpMin_State f s k e le) m c2' m2'.
+        match_cores (CSharpMin_State f s k e lenv) j (CSharpMin_State f s k e lenv) m c2' m2'.
+(*   exists c' : CSharpMin_core,
+        inj_match_states_star unit match_cores MC_measure (tt,c') j (CSharpMin_State f s k e lenv) m c2' m2'.*)
 Proof. intros.
   dependent induction MK.
 
@@ -323,37 +338,38 @@ Proof. intros.
   split.
     apply corestep_plus_one. 
         eapply CompCertStep_CMin_corestep'.  simpl.  econstructor. reflexivity.
-  simpl. exists (CSharpMin_State f s k e le).
-     left. eapply MC_states; eauto.
+  simpl. (* exists (CSharpMin_State f s k e le).
+     left. *) eapply MC_states; eauto.
  
   eexists. eexists.
   split.
     apply corestep_plus_one. 
         eapply CompCertStep_CMin_corestep'.  simpl.  econstructor. reflexivity.
-   simpl. exists (CSharpMin_State f (Csharpminor.Sseq s1 s2) k e le).
-      left.  eapply MC_state_seq; eauto.
+   simpl. (*exists (CSharpMin_State f (Csharpminor.Sseq s1 s2) k e le).
+      left.  *) eapply MC_state_seq; eauto.
 
-  exploit IHMK; eauto. clear IHMK.  intros [T2 [m2 [A [c' C]]]].
+  exploit IHMK; eauto. clear IHMK.  intros [T2 [m2 [A C]]].
   exists T2; exists m2.
   split.
      eapply corestep_star_plus_trans.
         apply corestep_star_one.  eapply CompCertStep_CMin_corestep'.  simpl.  constructor. reflexivity.
         simpl. apply A. 
-  simpl in *. exists c'. apply C.
+  apply C.
 Qed.
 
 Lemma MS_step_case_SkipBlock: 
-forall cenv sz f tfn j m tm e le te sp lo hi cs k tk xenv 
+forall cenv sz f tfn j m tm e lenv te sp lo hi cs k tk xenv 
 (TRF : transl_funbody cenv sz f = OK tfn)
 (MINJ : Mem.inject j m tm)
 (MK : match_cont (Csharpminor.Kblock k) tk (fn_return f) cenv xenv cs)
-(MCS : match_callstack prog j m tm (Frame cenv tfn e le te sp lo hi :: cs)
+(MCS : match_callstack prog j m tm (Frame cenv tfn e lenv te sp lo hi :: cs)
         (Mem.nextblock m) (Mem.nextblock tm)),
 exists c2' : CMin_core,
   exists m2' : mem,
         corestep_plus CMin_core_sem tge (CMin_State tfn Sskip tk (Vptr sp Int.zero) te) tm c2' m2' /\
-exists c' : CSharpMin_core,
-        inj_match_states_star unit match_cores MC_measure (tt,c') j (CSharpMin_State f Csharpminor.Sskip k e le) m c2' m2'.
+         match_cores  (CSharpMin_State f Csharpminor.Sskip k e lenv)   j (CSharpMin_State f Csharpminor.Sskip k e lenv) m c2' m2'
+(*exists c' : CSharpMin_core,
+        inj_match_states_star unit match_cores MC_measure (tt,c') j (CSharpMin_State f Csharpminor.Sskip k e le) m c2' m2'*).
 Proof. intros.
   dependent induction MK.
 
@@ -361,16 +377,16 @@ Proof. intros.
   split.
     apply corestep_plus_one. 
         eapply CompCertStep_CMin_corestep'.  simpl. constructor. reflexivity.  
-   simpl. exists (CSharpMin_State f Csharpminor.Sskip k e le).
-      left.  eapply MC_states; eauto.
+   simpl. (*exists (CSharpMin_State f Csharpminor.Sskip k e le).
+      left.  *) eapply MC_states; eauto.
 
-  exploit IHMK; eauto. clear IHMK.  intros [T2 [m2 [A [c' C]]]].
+  exploit IHMK; eauto. clear IHMK.  intros [T2 [m2 [A C]]].
   exists T2; exists m2.
   split.
      eapply corestep_star_plus_trans.
         apply corestep_star_one.  eapply CompCertStep_CMin_corestep'.  simpl.  constructor. reflexivity.
         simpl. apply A. 
-  simpl in *. exists c'. apply C.
+  (* simpl in *. exists c'.*) apply C.
 Qed.
 
 Lemma MS_match_is_call_cont:
@@ -394,20 +410,21 @@ Proof.
 Qed.
 
 Lemma MS_step_case_SkipCall:
- forall cenv sz f tfn j m tm e le te sp lo hi cs k tk xenv m'
+ forall cenv sz f tfn j m tm e lenv te sp lo hi cs k tk xenv m'
 (CC: Csharpminor.is_call_cont k)
 (RET: fn_return f = None)
 (FL: Mem.free_list m (blocks_of_env e) = Some m')
 (TRF : transl_funbody cenv sz f = OK tfn)
 (MINJ : Mem.inject j m tm)
 (MK : match_cont k tk (fn_return f) cenv xenv cs)
-(MCS : match_callstack prog j m tm (Frame cenv tfn e le te sp lo hi :: cs)
+(MCS : match_callstack prog j m tm (Frame cenv tfn e lenv te sp lo hi :: cs)
         (Mem.nextblock m) (Mem.nextblock tm)),
 exists c2' : CMin_core,
   exists m2' : mem,
         corestep_plus CMin_core_sem tge (CMin_State  tfn Sskip tk (Vptr sp Int.zero) te) tm c2' m2' /\
-exists c' : CSharpMin_core,
-       inj_match_states_star unit match_cores MC_measure (tt,c') j (CSharpMin_Returnstate Vundef k) m' c2' m2'.
+         match_cores  (CSharpMin_Returnstate Vundef k)  j (CSharpMin_Returnstate Vundef k) m' c2' m2'.
+(*exists c' : CSharpMin_core,
+       inj_match_states_star unit match_cores MC_measure (tt,c') j (CSharpMin_Returnstate Vundef k) m' c2' m2'.*)
 Proof. intros.
   exploit MS_match_is_call_cont; eauto. intros [tk' [A [B C]]]. 
   exploit match_callstack_freelist; eauto. intros [tm' [P [Q R]]].
@@ -419,68 +436,72 @@ Proof. intros.
     eauto.
     econstructor; eauto.
 
-  simpl in *. exists (CSharpMin_Returnstate Vundef k). left. econstructor; eauto.
+  simpl in *. (*exists (CSharpMin_Returnstate Vundef k). left. *) econstructor; eauto.
 Qed.
 
 Lemma MS_step_case_Assign:
-forall cenv sz f tfn j m tm e le te sp lo hi cs k tk xenv m' ts  x a x0 v id
-(EE:Csharpminor.eval_expr ge e le m a v)
+forall cenv sz f tfn j m tm e lenv te sp lo hi cs k tk xenv m' ts  x a x0 v id
+(EE:Csharpminor.eval_expr ge e lenv m a v)
 (ASS: exec_assign ge e m id v m')
 (TRF : transl_funbody cenv sz f = OK tfn)
 (MINJ : Mem.inject j m tm)
 (MK : match_cont k tk (fn_return f) cenv xenv cs)
-(MCS : match_callstack prog j m tm (Frame cenv tfn e le te sp lo hi :: cs)
+(MCS : match_callstack prog j m tm (Frame cenv tfn e lenv te sp lo hi :: cs)
         (Mem.nextblock m) (Mem.nextblock tm))
 (EQ : transl_expr cenv a = OK (x, x0))
 (EQ0 : var_set cenv id x = OK ts),
 exists c2' : CMin_core,
   exists m2' : mem,
         corestep_plus CMin_core_sem tge (CMin_State  tfn  ts tk (Vptr sp Int.zero) te) tm c2' m2' /\
-  exists c' : CSharpMin_core,
-       inj_match_states_star unit match_cores MC_measure (tt,c') j (CSharpMin_State f Csharpminor.Sskip k e le) m' c2' m2'.
+        match_cores (CSharpMin_State f Csharpminor.Sskip k e lenv) j (CSharpMin_State f Csharpminor.Sskip k e lenv) m' c2' m2'.
+(*  exists c' : CSharpMin_core,
+       inj_match_states_star unit match_cores MC_measure (tt,c') j (CSharpMin_State f Csharpminor.Sskip k e lenv) m' c2' m2'.*)
 Proof. intros.
   exploit transl_expr_correct; eauto. intros [tv [EVAL [VINJ APP]]].
   exploit var_set_correct; eauto. 
   intros [te' [tm' [EXEC [MINJ' [MCS' OTHER]]]]].
   eexists; eexists; split.
      apply corestep_plus_one. eapply CompCertStep_CMin_corestep'. eexact EXEC. reflexivity.
-  simpl in *. exists (CSharpMin_State f Csharpminor.Sskip k e le). left. econstructor; eauto.
+  simpl in *. (*exists (CSharpMin_State f Csharpminor.Sskip k e lenv). left. *) econstructor; eauto.
 Qed.
 
 Lemma MS_step_case_Set:
-forall cenv sz f tfn j m tm e le te sp lo hi cs k tk xenv x x0 v a id
-(H: Csharpminor.eval_expr ge e le m a v)
+forall cenv sz f tfn j m tm e lenv te sp lo hi cs k tk xenv x x0 v a id
+(H: Csharpminor.eval_expr ge e lenv m a v)
 (TRF : transl_funbody cenv sz f = OK tfn)
 (MINJ : Mem.inject j m tm)
-(MCS : match_callstack prog j m tm (Frame cenv tfn e le te sp lo hi :: cs)
+(MCS : match_callstack prog j m tm (Frame cenv tfn e lenv te sp lo hi :: cs)
         (Mem.nextblock m) (Mem.nextblock tm))
 (MK : match_cont k tk (fn_return f) cenv xenv cs)
 (EQ : transl_expr cenv a = OK (x, x0)),
 exists c2' : CMin_core,
   exists m2' : mem,
         corestep_plus CMin_core_sem tge (CMin_State  tfn (Sassign (for_temp id) x) tk (Vptr sp Int.zero) te) tm c2' m2' /\
-  exists c' : CSharpMin_core,
+       match_cores (CSharpMin_State f Csharpminor.Sskip k e (PTree.set id v lenv)) j 
+          (CSharpMin_State f Csharpminor.Sskip k e (PTree.set id v lenv)) m c2' m2' .
+(*  exists c' : CSharpMin_core,
         inj_match_states_star unit match_cores MC_measure (tt,c') j 
-          (CSharpMin_State f Csharpminor.Sskip k e (PTree.set id v le)) m c2' m2' .
+          (CSharpMin_State f Csharpminor.Sskip k e (PTree.set id v lenv)) m c2' m2' .*)
 Proof. intros.
   exploit transl_expr_correct; eauto. intros [tv [EVAL [VINJ APP]]].
   eexists; eexists; split.
      apply corestep_plus_one. eapply CompCertStep_CMin_corestep'. econstructor; eauto.  reflexivity.
   simpl in *.
-  assert (X:= match_callstack_set_temp _ _ _ _ _ _ _ _ _ _ _ _ _ _ _ id _ _ VINJ MCS).
-  exists (CSharpMin_State f Csharpminor.Sskip k e (PTree.set id v le)).
-    left. econstructor; eauto.
+  econstructor; eauto.
+  apply (match_callstack_set_temp _ _ _ _ _ _ _ _ _ _ _ _ _ _ _ id _ _ VINJ MCS).
+(*  exists (CSharpMin_State f Csharpminor.Sskip k e (PTree.set id v lenv)).
+    left. econstructor; eauto.*)
 Qed.
 
 Lemma MS_step_case_Store:
-forall cenv sz f tfn j m tm e le te sp lo hi cs k tk xenv x x0 x1 x2 
+forall cenv sz f tfn j m tm e lenv te sp lo hi cs k tk xenv x x0 x1 x2 
       chunk m' a addr vaddr v
 (CH: Mem.storev chunk m vaddr v = Some m')
-(EvAddr : Csharpminor.eval_expr ge e le m addr vaddr)
-(EvA : Csharpminor.eval_expr ge e le m a v)
+(EvAddr : Csharpminor.eval_expr ge e lenv m addr vaddr)
+(EvA : Csharpminor.eval_expr ge e lenv m a v)
 (TRF : transl_funbody cenv sz f = OK tfn)
 (MINJ : Mem.inject j m tm)
-(MCS : match_callstack prog j m tm (Frame cenv tfn e le te sp lo hi :: cs)
+(MCS : match_callstack prog j m tm (Frame cenv tfn e lenv te sp lo hi :: cs)
                 (Mem.nextblock m) (Mem.nextblock tm))
 (MK : match_cont k tk (fn_return f) cenv xenv cs)
 (EQ : transl_expr cenv addr = OK (x, x0))
@@ -488,9 +509,11 @@ forall cenv sz f tfn j m tm e le te sp lo hi cs k tk xenv x x0 x1 x2
 exists c2' : CMin_core,
   exists m2' : mem,
         corestep_plus CMin_core_sem tge (CMin_State  tfn (make_store chunk x x1) tk (Vptr sp Int.zero) te) tm c2' m2' /\
- exists c' : CSharpMin_core,
+        match_cores (CSharpMin_State f Csharpminor.Sskip k e lenv) j 
+                      (CSharpMin_State f Csharpminor.Sskip k e lenv) m' c2' m2' .
+(* exists c' : CSharpMin_core,
         inj_match_states_star unit match_cores MC_measure (tt,c') j 
-                      (CSharpMin_State f Csharpminor.Sskip k e le) m' c2' m2' .
+                      (CSharpMin_State f Csharpminor.Sskip k e lenv) m' c2' m2' .*)
 Proof. intros.
   exploit transl_expr_correct. eauto. eauto. eauto. eexact EvAddr. eauto. 
   intros [tv1 [EVAL1 [VINJ1 APP1]]].
@@ -501,22 +524,23 @@ Proof. intros.
   eexists; eexists; split.
       apply corestep_plus_one. eapply CompCertStep_CMin_corestep'. eexact EXEC. reflexivity.
   simpl in *.
-    assert (X:= match_callstack_storev_mapped _ _ _ _ _ _ _ _ _ _ _  VINJ1 CH STORE' _ _ _ MCS).
-    exists (CSharpMin_State f Csharpminor.Sskip k e le).
-    left. econstructor; eauto.
+(*    assert (X:= match_callstack_storev_mapped _ _ _ _ _ _ _ _ _ _ _  VINJ1 CH STORE' _ _ _ MCS).
+    exists (CSharpMin_State f Csharpminor.Sskip k e lenv).
+    left.*) econstructor; eauto.
+      eapply match_callstack_storev_mapped. eexact VINJ1. eauto. eauto.
       rewrite (nextblock_storev _ _ _ _ _ CH).
       rewrite (nextblock_storev _ _ _ _ _ STORE').
       eauto.
 Qed. 
 
 Lemma MS_step_case_Call:
-forall cenv sz f tfn j m tm e le te sp lo hi cs k tk xenv  x x0 x1 a vf fd optid vargs bl
-(EvalA: Csharpminor.eval_expr ge e le m a vf)
-(EvalBL: Csharpminor.eval_exprlist ge e le m bl vargs)
+forall cenv sz f tfn j m tm e lenv te sp lo hi cs k tk xenv  x x0 x1 a vf fd optid vargs bl
+(EvalA: Csharpminor.eval_expr ge e lenv m a vf)
+(EvalBL: Csharpminor.eval_exprlist ge e lenv m bl vargs)
 (FF: Genv.find_funct ge vf = Some fd)
 (TRF : transl_funbody cenv sz f = OK tfn)
 (MINJ : Mem.inject j m tm)
-(MCS : match_callstack prog j m tm (Frame cenv tfn e le te sp lo hi :: cs)
+(MCS : match_callstack prog j m tm (Frame cenv tfn e lenv te sp lo hi :: cs)
         (Mem.nextblock m) (Mem.nextblock tm))
 (MK : match_cont tk k (fn_return f) cenv xenv cs)
 (EQ : transl_expr cenv a = OK (x, x0))
@@ -524,10 +548,12 @@ forall cenv sz f tfn j m tm e le te sp lo hi cs k tk xenv  x x0 x1 a vf fd optid
 exists c2' : CMin_core,
   exists m2' : mem,
         corestep_plus CMin_core_sem tge 
-           (CMin_State  tfn (Scall (option_map for_temp optid) (Csharpminor.funsig fd) x x1)  k (Vptr sp Int.zero) te) tm c2' m2' /\
- exists c' : CSharpMin_core,
+             (CMin_State  tfn (Scall (option_map for_temp optid) (Csharpminor.funsig fd) x x1)  k (Vptr sp Int.zero) te) tm c2' m2' /\
+       match_cores (CSharpMin_Callstate fd vargs (Csharpminor.Kcall optid f e lenv tk))  j
+              (CSharpMin_Callstate fd vargs (Csharpminor.Kcall optid f e lenv tk)) m c2' m2'.
+(* exists c' : CSharpMin_core,
         inj_match_states_star unit match_cores MC_measure (tt,c') j
-              (CSharpMin_Callstate fd vargs (Csharpminor.Kcall optid f e le tk)) m c2' m2'.
+              (CSharpMin_Callstate fd vargs (Csharpminor.Kcall optid f e lenv tk)) m c2' m2'.*)
 Proof. intros.
   simpl in FF. exploit functions_translated; eauto. intros [tfd [FIND TRANS]].
   exploit transl_expr_correct; eauto. intros [tvf [EVAL1 [VINJ1 APP1]]].
@@ -543,19 +569,19 @@ Proof. intros.
                       eapply sig_preserved; eauto.
           econstructor; eauto.
   simpl in *.
-     exists  (CSharpMin_Callstate fd vargs (Csharpminor.Kcall optid f e le tk)).
-     left. econstructor; eauto. eapply match_Kcall with (cenv' := cenv); eauto.
+     (*exists  (CSharpMin_Callstate fd vargs (Csharpminor.Kcall optid f e lenv tk)).
+     left.*) econstructor; eauto. eapply match_Kcall with (cenv' := cenv); eauto.
             simpl; trivial.
-      admit. admit. (*These are the new conditions in rule MC_Callstate*)
+      admit. admit. (*These are the new conditions in rulenv MC_Callstate*)
 Qed.
 
 Lemma MS_step_case_Builtin:
-forall cenv sz f tfn j m tm e le te sp lo hi cs k tk xenv x t ef optid vres m' bl vargs
-(EvalArgs: Csharpminor.eval_exprlist ge e le m bl vargs)
+forall cenv sz f tfn j m tm e lenv te sp lo hi cs k tk xenv x t ef optid vres m' bl vargs
+(EvalArgs: Csharpminor.eval_exprlist ge e lenv m bl vargs)
 (ExtCall: Events.external_call ef ge vargs m t vres m')
 (TRF : transl_funbody cenv sz f = OK tfn)
 (MINJ : Mem.inject j m tm)
-(MCS : match_callstack prog j m tm (Frame cenv tfn e le te sp lo hi :: cs)
+(MCS : match_callstack prog j m tm (Frame cenv tfn e lenv te sp lo hi :: cs)
         (Mem.nextblock m) (Mem.nextblock tm))
 (MK : match_cont k tk (fn_return f) cenv xenv cs)
 (EQ : transl_exprlist cenv bl = OK x),
@@ -566,9 +592,11 @@ exists c2' : CMin_core,
   exists j' : meminj,
         inject_incr j j' /\
         Events.inject_separated j j' m tm /\
-  exists c',
+       match_cores (CSharpMin_State f Csharpminor.Sskip k e (set_optvar optid vres lenv))  j'
+              (CSharpMin_State f Csharpminor.Sskip k e (set_optvar optid vres lenv)) m' c2' m2'.
+(*  exists c',
         inj_match_states_star unit match_cores MC_measure (tt,c') j'
-          (CSharpMin_State f Csharpminor.Sskip k e (set_optvar optid vres le)) m' c2' m2'.
+          (CSharpMin_State f Csharpminor.Sskip k e (set_optvar optid vres lenv)) m' c2' m2'.*)
 Proof. intros.
   exploit transl_exprlist_correct; eauto.
   intros [tvargs [EVAL2 VINJ2]].
@@ -585,7 +613,7 @@ Proof. intros.
                  eapply var_info_rev_translated; assumption.
            reflexivity.
   assert (MCS': match_callstack prog j' m' tm'
-                 (Frame cenv tfn e le te sp lo hi :: cs)
+                 (Frame cenv tfn e lenv te sp lo hi :: cs)
                  (Mem.nextblock m') (Mem.nextblock tm')).
     apply match_callstack_incr_bound with (Mem.nextblock m) (Mem.nextblock tm).
     eapply match_callstack_external_call; eauto.
@@ -594,8 +622,8 @@ Proof. intros.
     eapply external_call_nextblock_incr; eauto.
     eapply external_call_nextblock_incr; eauto.
 exists j'. split. assumption.  split. assumption. 
-  simpl in *. exists  (CSharpMin_State f Csharpminor.Sskip k e (set_optvar optid vres le)).
-  left. econstructor; eauto.
+  simpl in *. (* exists  (CSharpMin_State f Csharpminor.Sskip k e (set_optvar optid vres lenv)).
+  left. *) econstructor; eauto.
 Opaque PTree.set.
   unfold set_optvar. destruct optid; simpl. 
   eapply match_callstack_set_temp; eauto. 
@@ -603,12 +631,12 @@ Opaque PTree.set.
 Qed.
 
 Lemma MS_step_case_Ite: 
-forall cenv sz f tfn j m tm e le te sp lo hi cs k tk xenv x x0 x1 x2 b v a s1 s2
-(H : Csharpminor.eval_expr ge e le m a v)
+forall cenv sz f tfn j m tm e lenv te sp lo hi cs k tk xenv x x0 x1 x2 b v a s1 s2
+(H : Csharpminor.eval_expr ge e lenv m a v)
 (BoolOfVal : Val.bool_of_val v b)
 (TRF : transl_funbody cenv sz f = OK tfn)
 (MINJ : Mem.inject j m tm)
-(MCS : match_callstack prog j m tm (Frame cenv tfn e le te sp lo hi :: cs)
+(MCS : match_callstack prog j m tm (Frame cenv tfn e lenv te sp lo hi :: cs)
         (Mem.nextblock m) (Mem.nextblock tm))
 (MK : match_cont k tk (fn_return f) cenv xenv cs)
 (EQ : transl_expr cenv a = OK (x, x0))
@@ -618,9 +646,11 @@ exists c2' : CMin_core,
   exists m2' : mem,
         corestep_plus CMin_core_sem tge
              (CMin_State tfn (Sifthenelse x x1 x2) tk (Vptr sp Int.zero) te) tm c2' m2' /\
-  exists c',
+        match_cores  (CSharpMin_State f (if b then s1 else s2) k e lenv)  j
+             (CSharpMin_State f (if b then s1 else s2) k e lenv) m c2' m2'.
+(*  exists c',
         inj_match_states_star unit match_cores MC_measure (tt,c') j
-             (CSharpMin_State f (if b then s1 else s2) k e le) m c2' m2'.
+             (CSharpMin_State f (if b then s1 else s2) k e lenv) m c2' m2'.*)
 Proof. intros.
   exploit transl_expr_correct; eauto. intros [tv [EVAL [VINJ APP]]].
   exists (CMin_State tfn (if b then x1 else x2) tk (Vptr sp Int.zero) te). exists tm.
@@ -629,24 +659,26 @@ Proof. intros.
               eapply step_ifthenelse; eauto. eapply bool_of_val_inject; eauto.
         econstructor; eauto.
   simpl in *.
-    exists (CSharpMin_State f (if b then s1 else s2) k e le).
-    left. econstructor; eauto.
+ (*   exists (CSharpMin_State f (if b then s1 else s2) k e lenv).
+    left. *) econstructor; eauto.
        destruct b; auto.
 Qed.
 
 Lemma MS_step_case_Loop:
-forall cenv sz f tfn j m tm e le te sp lo hi cs k tk xenv x s
+forall cenv sz f tfn j m tm e lenv te sp lo hi cs k tk xenv x s
 (TRF : transl_funbody cenv sz f = OK tfn)
 (MINJ : Mem.inject j m tm)
-(MCS : match_callstack prog j m tm (Frame cenv tfn e le te sp lo hi :: cs)
+(MCS : match_callstack prog j m tm (Frame cenv tfn e lenv te sp lo hi :: cs)
         (Mem.nextblock m) (Mem.nextblock tm))
 (MK : match_cont tk k (fn_return f) cenv xenv cs)
 (EQ : transl_stmt (fn_return f) cenv xenv s = OK x),
 exists c2' : CMin_core,
   exists m2' : mem,
       corestep_plus CMin_core_sem tge (CMin_State tfn (Sloop x) k (Vptr sp Int.zero) te) tm c2' m2' /\
-    exists c',   inj_match_states_star unit match_cores MC_measure (tt,c') j
-          (CSharpMin_State f s (Csharpminor.Kseq (Csharpminor.Sloop s) tk) e le) m c2' m2'. 
+      match_cores  (CSharpMin_State f s (Csharpminor.Kseq (Csharpminor.Sloop s) tk) e lenv)  j
+          (CSharpMin_State f s (Csharpminor.Kseq (Csharpminor.Sloop s) tk) e lenv) m c2' m2'. 
+(*    exists c',   inj_match_states_star unit match_cores MC_measure (tt,c') j
+          (CSharpMin_State f s (Csharpminor.Kseq (Csharpminor.Sloop s) tk) e lenv) m c2' m2'. *)
 Proof. intros.
   eexists; eexists.
   split.
@@ -654,48 +686,51 @@ Proof. intros.
         econstructor; eauto.
         reflexivity.
   simpl in *.
-      exists  (CSharpMin_State f s (Csharpminor.Kseq (Csharpminor.Sloop s) tk) e le).
-      left.
+(*      exists  (CSharpMin_State f s (Csharpminor.Kseq (Csharpminor.Sloop s) tk) e lenv).
+      left.*)
       econstructor; eauto. econstructor; eauto. simpl. rewrite EQ; auto. 
 Qed.
 
 Lemma MS_step_case_Block:
-forall cenv sz f tfn j m tm e le te sp lo hi cs k tk xenv x s
+forall cenv sz f tfn j m tm e lenv te sp lo hi cs k tk xenv x s
 (TRF : transl_funbody cenv sz f = OK tfn)
 (MINJ : Mem.inject j m tm)
-(MCS : match_callstack prog j m tm (Frame cenv tfn e le te sp lo hi :: cs)
+(MCS : match_callstack prog j m tm (Frame cenv tfn e lenv te sp lo hi :: cs)
         (Mem.nextblock m) (Mem.nextblock tm))
 (MK : match_cont tk k (fn_return f) cenv xenv cs)
 (EQ : transl_stmt (fn_return f) cenv (true :: xenv) s = OK x),
 exists c2' : CMin_core,
   exists m2' : mem,
         corestep_plus CMin_core_sem tge (CMin_State tfn (Sblock x) k (Vptr sp Int.zero) te) tm c2' m2' /\
-    exists c' ,
-       inj_match_states_star unit match_cores MC_measure (tt,c') j (CSharpMin_State f s (Csharpminor.Kblock tk) e le) m c2' m2'.
+        match_cores (CSharpMin_State f s (Csharpminor.Kblock tk) e lenv)  j (CSharpMin_State f s (Csharpminor.Kblock tk) e lenv) m c2' m2'.
+(*    exists c' ,
+       inj_match_states_star unit match_cores MC_measure (tt,c') j (CSharpMin_State f s (Csharpminor.Kblock tk) e lenv) m c2' m2'.*)
 Proof. intros.
   eexists; eexists; split.
      apply corestep_plus_one. eapply CompCertStep_CMin_corestep'.
         econstructor; eauto.
         reflexivity.
   simpl in *.
-      exists  (CSharpMin_State f s (Csharpminor.Kblock tk) e le).
-      left.
+(*      exists  (CSharpMin_State f s (Csharpminor.Kblock tk) e lenv).
+      left.*)
       econstructor; eauto. econstructor; eauto. 
 Qed.
 
 Lemma MS_step_case_ExitSeq:
-forall  cenv sz f tfn j m tm e le te sp lo hi cs k tk xenv n s
+forall  cenv sz f tfn j m tm e lenv te sp lo hi cs k tk xenv n s
 (TRF : transl_funbody cenv sz f = OK tfn)
 (MINJ : Mem.inject j m tm)
-(MCS : match_callstack prog j m tm (Frame cenv tfn e le te sp lo hi :: cs)
+(MCS : match_callstack prog j m tm (Frame cenv tfn e lenv te sp lo hi :: cs)
         (Mem.nextblock m) (Mem.nextblock tm))
 (MK : match_cont (Csharpminor.Kseq s tk) k (fn_return f) cenv xenv cs),
 exists c2' : CMin_core,
   exists m2' : mem,
         corestep_plus CMin_core_sem tge
                (CMin_State tfn (Sexit (shift_exit xenv n)) k (Vptr sp Int.zero) te) tm c2' m2'  /\
-    exists c',  inj_match_states_star unit match_cores MC_measure (tt,c') j
-                                   (CSharpMin_State f (Csharpminor.Sexit n) tk e le) m c2' m2'.
+        match_cores (CSharpMin_State f (Csharpminor.Sexit n) tk e lenv) j
+                               (CSharpMin_State f (Csharpminor.Sexit n) tk e lenv) m c2' m2'.
+(*    exists c',  inj_match_states_star unit match_cores MC_measure (tt,c') j
+                                   (CSharpMin_State f (Csharpminor.Sexit n) tk e lenv) m c2' m2'.*)
 Proof. intros.
   dependent induction MK.
 
@@ -704,8 +739,8 @@ Proof. intros.
         econstructor; eauto.
         reflexivity.
   simpl in *.
-      exists   (CSharpMin_State f (Csharpminor.Sexit n) tk e le).
-      left. econstructor; eauto. reflexivity.
+      (*exists   (CSharpMin_State f (Csharpminor.Sexit n) tk e lenv).
+      left.*) econstructor; eauto. reflexivity.
 
   exploit IHMK; eauto. intros [c2' [m2' [A B]]].
   exists c2'. exists m2'. 
@@ -723,25 +758,27 @@ Proof. intros.
 Qed.
 
 Lemma MS_step_case_ExitBlockZero:
-forall  cenv sz f tfn j m tm e le te sp lo hi cs k tk xenv 
+forall  cenv sz f tfn j m tm e lenv te sp lo hi cs k tk xenv 
 (TRF : transl_funbody cenv sz f = OK tfn)
 (MINJ : Mem.inject j m tm)
-(MCS : match_callstack prog j m tm (Frame cenv tfn e le te sp lo hi :: cs)
+(MCS : match_callstack prog j m tm (Frame cenv tfn e lenv te sp lo hi :: cs)
         (Mem.nextblock m) (Mem.nextblock tm))
 (MK : match_cont (Csharpminor.Kblock tk) k (fn_return f) cenv xenv cs),
 exists c2' : CMin_core,
   exists m2' : mem,
        corestep_plus CMin_core_sem tge (CMin_State tfn (Sexit (shift_exit xenv 0)) k (Vptr sp Int.zero) te) tm c2' m2' /\
-    exists c', inj_match_states_star unit match_cores MC_measure (tt,c') j
-                                    (CSharpMin_State f Csharpminor.Sskip tk e le) m c2' m2'.
+       match_cores  (CSharpMin_State f Csharpminor.Sskip tk e lenv) j
+                              (CSharpMin_State f Csharpminor.Sskip tk e lenv) m c2' m2'.
+(*    exists c', inj_match_states_star unit match_cores MC_measure (tt,c') j
+                                    (CSharpMin_State f Csharpminor.Sskip tk e lenv) m c2' m2'.*)
 Proof. intros.
   dependent induction MK.
 
   eexists; eexists; split.
      apply corestep_plus_one. eapply CompCertStep_CMin_corestep'. constructor. reflexivity. 
   simpl in *.
-    exists  (CSharpMin_State f Csharpminor.Sskip tk e le). 
-    left. econstructor; eauto.
+    (*exists  (CSharpMin_State f Csharpminor.Sskip tk e lenv). 
+    left.*) econstructor; eauto.
 
   exploit IHMK; eauto. intros [c2' [m2' [A B]]].
   exists c2'. exists m2'. 
@@ -752,26 +789,25 @@ Proof. intros.
 Qed.
 
 Lemma MS_step_case_ExitBlockNonzero:
-forall  cenv sz f tfn j m tm e le te sp lo hi cs k tk xenv n
+forall  cenv sz f tfn j m tm e lenv te sp lo hi cs k tk xenv n
 (TRF : transl_funbody cenv sz f = OK tfn)
 (MINJ : Mem.inject j m tm)
-(MCS : match_callstack prog j m tm (Frame cenv tfn e le te sp lo hi :: cs)
+(MCS : match_callstack prog j m tm (Frame cenv tfn e lenv te sp lo hi :: cs)
                      (Mem.nextblock m) (Mem.nextblock tm))
 (MK : match_cont (Csharpminor.Kblock tk) k (fn_return f) cenv xenv cs),
 exists c2' : CMin_core,
   exists m2' : mem,
         corestep_plus CMin_core_sem tge
                      (CMin_State tfn (Sexit (shift_exit xenv (S n))) k (Vptr sp Int.zero) te) tm c2' m2' /\ 
-    exists c', inj_match_states_star unit match_cores MC_measure (tt,c') j
-          (CSharpMin_State f (Csharpminor.Sexit n) tk e le) m c2' m2'.
+       match_cores (CSharpMin_State f (Csharpminor.Sexit n) tk e lenv)  j
+          (CSharpMin_State f (Csharpminor.Sexit n) tk e lenv) m c2' m2'.
 Proof. intros.
   dependent induction MK.
 
   eexists; eexists; split.
      apply corestep_plus_one. eapply CompCertStep_CMin_corestep'. constructor. reflexivity. 
   simpl in *.
-    exists  (CSharpMin_State f (Csharpminor.Sexit n) tk e le).
-    left. econstructor; eauto. auto.
+    econstructor; eauto. auto.
 
   exploit IHMK; eauto. intros [c2' [m2' [A B]]].
   exists c2'. exists m2'. 
@@ -838,18 +874,18 @@ Proof.
 Qed.
 
 Lemma MS_switch_MSI:
-  forall fn k e le m tfn ts tk sp te tm cenv xenv j lo hi cs sz ls body tk'
+  forall fn k e lenv m tfn ts tk sp te tm cenv xenv j lo hi cs sz ls body tk'
     (TRF: transl_funbody cenv sz fn = OK tfn)
     (TR: transl_lblstmt (fn_return fn) cenv (switch_env ls xenv) ls body = OK ts)
     (MINJ: Mem.inject j m tm)
     (MCS: match_callstack prog j m tm
-               (Frame cenv tfn e le te sp lo hi :: cs)
+               (Frame cenv tfn e lenv te sp lo hi :: cs)
                (Mem.nextblock m) (Mem.nextblock tm))
     (MK: match_cont k tk (fn_return fn) cenv xenv cs)
     (TK: transl_lblstmt_cont (fn_return fn) cenv xenv ls tk tk'),
   exists S, exists mm,
   corestep_plus CMin_core_sem tge (CMin_State tfn (Sexit O) tk' (Vptr sp Int.zero) te) tm S mm
-  /\ match_statesInj prog j (Csharpminor.State fn (seq_of_lbl_stmt ls) k e le m) (Cminor_CompcertSemantics.ToState S mm).
+  /\ match_statesInj prog j (Csharpminor.State fn (seq_of_lbl_stmt ls) k e lenv m) (Cminor_CompcertSemantics.ToState S mm).
 Proof.
   intros. destruct ls; simpl.
 (*1*)
@@ -869,11 +905,11 @@ Proof.
 Qed.
 
 Lemma MS_step_case_Switch:
-forall cenv sz f tfn j m tm e le te sp lo hi cs k tk xenv a x x0 ts cases n
-(EvalA: Csharpminor.eval_expr ge e le m a (Vint n))
+forall cenv sz f tfn j m tm e lenv te sp lo hi cs k tk xenv a x x0 ts cases n
+(EvalA: Csharpminor.eval_expr ge e lenv m a (Vint n))
 (TRF : transl_funbody cenv sz f = OK tfn)
 (MINJ : Mem.inject j m tm)
-(MCS : match_callstack prog j m tm (Frame cenv tfn e le te sp lo hi :: cs)
+(MCS : match_callstack prog j m tm (Frame cenv tfn e lenv te sp lo hi :: cs)
         (Mem.nextblock m) (Mem.nextblock tm))
 (MK : match_cont k tk (fn_return f) cenv xenv cs)
 (EQ : transl_expr cenv a = OK (x, x0))
@@ -883,7 +919,8 @@ forall cenv sz f tfn j m tm e le te sp lo hi cs k tk xenv a x x0 ts cases n
 exists c2' : CMin_core,
   exists m2' : mem,
           corestep_plus CMin_core_sem tge (CMin_State tfn ts tk (Vptr sp Int.zero) te) tm c2' m2' /\
-    exists c', inj_match_states_star unit match_cores MC_measure (tt,c') j (CSharpMin_State f (seq_of_lbl_stmt (select_switch n cases)) k e le) m c2' m2'.
+         match_cores (CSharpMin_State f (seq_of_lbl_stmt (select_switch n cases)) k e lenv)  j
+                               (CSharpMin_State f (seq_of_lbl_stmt (select_switch n cases)) k e lenv) m c2' m2'.
 Proof. intros.
   exploit transl_expr_correct; eauto. intros [tv [EVAL [VINJ APP]]].
   inv VINJ.
@@ -900,47 +937,44 @@ Proof. intros.
         eapply corestep_star_trans.
          apply C.
          eapply corestep_plus_star. eapply F.
-  exists (CSharpMin_State f (seq_of_lbl_stmt (select_switch n cases)) k e le).
-   left. simpl. eapply MSI_MC. apply G.
+  simpl. eapply MSI_MC. apply G.
 Qed.
 
 Lemma MS_step_case_ReturnNone:
-forall cenv sz f tfn j m tm e le te sp lo hi cs k tk xenv m'
+forall cenv sz f tfn j m tm e lenv te sp lo hi cs k tk xenv m'
 (Freelist: Mem.free_list m (blocks_of_env e) = Some m')
 (TRF : transl_funbody cenv sz f = OK tfn)
 (MINJ : Mem.inject j m tm)
-(MCS : match_callstack prog j m tm (Frame cenv tfn e le te sp lo hi :: cs)
+(MCS : match_callstack prog j m tm (Frame cenv tfn e lenv te sp lo hi :: cs)
                  (Mem.nextblock m) (Mem.nextblock tm))
 (MK : match_cont tk k (fn_return f) cenv xenv cs),
 exists c2' : CMin_core,
   exists m2' : mem,
         corestep_plus CMin_core_sem tge (CMin_State tfn (Sreturn None) k (Vptr sp Int.zero) te) tm c2' m2'  /\
-    exists c', inj_match_states_star unit match_cores MC_measure (tt,c') j
+       match_cores (CSharpMin_Returnstate Vundef (Csharpminor.call_cont tk))  j
                              (CSharpMin_Returnstate Vundef (Csharpminor.call_cont tk)) m' c2' m2'.
 Proof. intros.
   exploit match_callstack_freelist; eauto. intros [tm' [A [B C]]].
   eexists; eexists; split.
      apply corestep_plus_one. eapply CompCertStep_CMin_corestep'. eapply step_return_0. eauto. reflexivity. 
   simpl in *.
-    exists (CSharpMin_Returnstate Vundef (Csharpminor.call_cont tk)).
-    left. econstructor; eauto. eapply match_call_cont; eauto.
+    econstructor; eauto. eapply match_call_cont; eauto.
 Qed.
 
 Lemma MS_step_case_ReturnSome:
-forall cenv sz f tfn j m tm e le te sp lo hi cs k tk xenv a x x0 m' v 
-(EvalA: Csharpminor.eval_expr ge e le m a v)
+forall cenv sz f tfn j m tm e lenv te sp lo hi cs k tk xenv a x x0 m' v 
+(EvalA: Csharpminor.eval_expr ge e lenv m a v)
 (Freelist: Mem.free_list m (blocks_of_env e) = Some m')
 (TRF : transl_funbody cenv sz f = OK tfn)
 (MINJ : Mem.inject j m tm)
-(MCS : match_callstack prog j m tm (Frame cenv tfn e le te sp lo hi :: cs)
+(MCS : match_callstack prog j m tm (Frame cenv tfn e lenv te sp lo hi :: cs)
         (Mem.nextblock m) (Mem.nextblock tm))
 (MK : match_cont tk k (fn_return f) cenv xenv cs)
 (EQ : transl_expr cenv a = OK (x, x0)),
 exists c2' : CMin_core,
   exists m2' : mem,
         corestep_plus CMin_core_sem tge (CMin_State tfn (Sreturn (Some x)) k (Vptr sp Int.zero) te) tm c2' m2' /\
-    exists c' ,
-          inj_match_states_star unit match_cores MC_measure (tt,c') j
+        match_cores  (CSharpMin_Returnstate v (Csharpminor.call_cont tk)) j
                  (CSharpMin_Returnstate v (Csharpminor.call_cont tk)) m' c2' m2'.
 Proof. intros.
   exploit transl_expr_correct; eauto. intros [tv [EVAL [VINJ APP]]].
@@ -948,58 +982,56 @@ Proof. intros.
   eexists; eexists; split.
      apply corestep_plus_one. eapply CompCertStep_CMin_corestep'. eapply step_return_1. eauto. eauto. reflexivity. 
   simpl in *.
-    exists  (CSharpMin_Returnstate v (Csharpminor.call_cont tk)).
-    left. econstructor; eauto. eapply match_call_cont; eauto.
+    econstructor; eauto. eapply match_call_cont; eauto.
 Qed.
 
 Lemma MS_step_case_Label:
-forall cenv sz f tfn j m tm e le te sp lo hi cs k tk xenv lbl x s
+forall cenv sz f tfn j m tm e lenv te sp lo hi cs k tk xenv lbl x s
 (TRF : transl_funbody cenv sz f = OK tfn)
 (MINJ : Mem.inject j m tm)
-(MCS : match_callstack prog j m tm (Frame cenv tfn e le te sp lo hi :: cs)
+(MCS : match_callstack prog j m tm (Frame cenv tfn e lenv te sp lo hi :: cs)
         (Mem.nextblock m) (Mem.nextblock tm))
 (MK : match_cont k tk (fn_return f) cenv xenv cs)
 (EQ : transl_stmt (fn_return f) cenv xenv s = OK x),
 exists c2' : CMin_core,
   exists m2' : mem,
        corestep_plus CMin_core_sem tge (CMin_State tfn (Slabel lbl x) tk (Vptr sp Int.zero) te) tm c2' m2' /\ 
-    exists c', inj_match_states_star unit match_cores MC_measure (tt,c') j (CSharpMin_State f s k e le) m c2' m2'.
+      match_cores (CSharpMin_State f s k e lenv)  j (CSharpMin_State f s k e lenv) m c2' m2'.
 Proof. intros.
   eexists; eexists; split.
     eapply corestep_plus_one. eapply CompCertStep_CMin_corestep'. constructor. reflexivity.
   simpl.
-  exists (CSharpMin_State f s k e le). 
-    left. econstructor; eauto.
+  econstructor; eauto.
 Qed.
 
 Lemma MS_step_case_Goto:
-forall cenv sz f tfn j m tm e le te sp lo hi cs k tk xenv lbl s' k'
+forall cenv sz f tfn j m tm e lenv te sp lo hi cs k tk xenv lbl s' k'
 (FindLab: Csharpminor.find_label lbl (Csharpminor.fn_body f)
        (Csharpminor.call_cont k) = Some (s', k'))
 (TRF : transl_funbody cenv sz f = OK tfn)
 (MINJ : Mem.inject j m tm)
-(MCS : match_callstack prog j m tm (Frame cenv tfn e le te sp lo hi :: cs)
+(MCS : match_callstack prog j m tm (Frame cenv tfn e lenv te sp lo hi :: cs)
         (Mem.nextblock m) (Mem.nextblock tm))
 (MK : match_cont k tk (fn_return f) cenv xenv cs),
 exists c2' : CMin_core,
   exists m2' : mem,
-          corestep_plus CMin_core_sem tge (CMin_State tfn (Sgoto lbl) tk (Vptr sp Int.zero) te) tm c2' m2' /\
-    exists c', inj_match_states_star unit match_cores MC_measure (tt,c') j (CSharpMin_State f s' k' e le) m c2' m2'.
+       corestep_plus CMin_core_sem tge (CMin_State tfn (Sgoto lbl) tk (Vptr sp Int.zero) te) tm c2' m2' /\
+       match_cores  (CSharpMin_State f s' k' e lenv) j (CSharpMin_State f s' k' e lenv) m c2' m2'.
 Proof. intros.
   exploit transl_find_label_body; eauto. 
   intros [ts' [tk' [xenv' [A [B C]]]]].
   eexists; eexists; split.
     eapply corestep_plus_one. eapply CompCertStep_CMin_corestep'. apply step_goto. eexact A. reflexivity.
   simpl.
-  exists (CSharpMin_State f s' k' e le).
-    left. econstructor; eauto.
+  econstructor; eauto.
 Qed.
+
 
 (******************************Functions required for internal call rule*****************************)
 (****These extend the original lemmas by additional guarantees of the (now exposed) memory injections, in order
     for the overall lemma for internal calls to establish the inject_separated fact******************************)
 Lemma MS_match_callstack_alloc_variable:
-  forall atk id lv cenv sz cenv' sz' tm sp e tf m m' b te le lo cs f tv,
+  forall atk id lv cenv sz cenv' sz' tm sp e tf m m' b te lenv lo cs f tv,
   assign_variable atk (id, lv) (cenv, sz) = (cenv', sz') ->
   Mem.valid_block tm sp ->
   (forall ofs k p,
@@ -1008,7 +1040,7 @@ Lemma MS_match_callstack_alloc_variable:
   tf.(fn_stackspace) <= Int.max_unsigned ->
   Mem.alloc m 0 (sizeof lv) = (m', b) ->
   match_callstack prog f m tm 
-                  (Frame cenv tf e le te sp lo (Mem.nextblock m) :: cs)
+                  (Frame cenv tf e lenv te sp lo (Mem.nextblock m) :: cs)
                   (Mem.nextblock m) (Mem.nextblock tm) ->
   Mem.inject f m tm ->
   0 <= sz -> sz' <= tf.(fn_stackspace) ->
@@ -1020,7 +1052,7 @@ Lemma MS_match_callstack_alloc_variable:
      inject_incr f f'
   /\ Mem.inject f' m' tm
   /\ match_callstack prog f' m' tm
-                     (Frame cenv' tf (PTree.set id (b, lv) e) le te sp lo (Mem.nextblock m') :: cs)
+                     (Frame cenv' tf (PTree.set id (b, lv) e) lenv te sp lo (Mem.nextblock m') :: cs)
                      (Mem.nextblock m') (Mem.nextblock tm)
   /\ (forall b delta ofs k p,
       f' b = Some(sp, delta) -> Mem.perm m' b ofs k p -> ofs + delta < sz') 
@@ -1124,7 +1156,7 @@ Proof.
 Qed.
 
 Lemma MS_match_callstack_alloc_variables_rec:
-  forall tm sp cenv' tf le te lo cs atk,
+  forall tm sp cenv' tf lenv te lo cs atk,
   Mem.valid_block tm sp ->
   (forall ofs k p,
     Mem.perm tm sp ofs k p -> 0 <= ofs < tf.(fn_stackspace)) ->
@@ -1135,7 +1167,7 @@ Lemma MS_match_callstack_alloc_variables_rec:
   forall f cenv sz,
   assign_variables atk vars (cenv, sz) = (cenv', tf.(fn_stackspace)) ->
   match_callstack prog f m tm 
-                  (Frame cenv tf e le te sp lo (Mem.nextblock m) :: cs)
+                  (Frame cenv tf e lenv te sp lo (Mem.nextblock m) :: cs)
                   (Mem.nextblock m) (Mem.nextblock tm) ->
   Mem.inject f m tm ->
   0 <= sz ->
@@ -1148,7 +1180,7 @@ Lemma MS_match_callstack_alloc_variables_rec:
      inject_incr f f'
   /\ Mem.inject f' m' tm
   /\ match_callstack prog f' m' tm
-                     (Frame cenv' tf e' le te sp lo (Mem.nextblock m') :: cs)
+                     (Frame cenv' tf e' lenv te sp lo (Mem.nextblock m') :: cs)
                      (Mem.nextblock m') (Mem.nextblock tm)
 (****************The following three conditions are new******************)
 (*** Note that in the third clause, we only "step" from m' to m ***************)
@@ -1173,7 +1205,7 @@ Proof.
     intros. eapply DEFINED. simpl. right. eauto.
   assert (exists tv, te!(for_var id) = Some tv).
     assert (te!(for_var id) <> None). eapply DEFINED. simpl; left; auto.
-    destruct (te!(for_var id)). exists v; auto. congruence.
+    destruct (te!(for_var id)). exists v; auto. exfalso. apply H1.  trivial. (*congruence. won;'t worlk here all of a sudden*)
   destruct H1 as [tv TEID].
   assert (sz1 <= fn_stackspace tf). eapply assign_variables_incr; eauto. 
   exploit MS_match_callstack_alloc_variable; eauto with coqlib.
@@ -1261,7 +1293,7 @@ exists f' ; intuition.
             assert (j' b = Some (b0,z)). apply (H6 _ _ _ Heqz). 
              rewrite H9 in H10; inv H10.
              assert (Z:= SP _ _ _ H8 Heqz); subst.
-             split; intros N. rewrite (VB1 _ N) in Heqz. congruence.
+             split; intros N. rewrite (VB1 _ N) in Heqz. rewrite Heqz in H8. inv H8. (*congruence again doesnt work here*)
              eapply (Mem.fresh_block_alloc _ _ _ _ _ H3 N).
   (*None*) assert (HH:= SEP _ H6 H7).
                      destruct (HH _ _ _ Heqz H9).
@@ -1270,9 +1302,9 @@ exists f' ; intuition.
 Qed.
 
 Lemma MS_var_set_self_correct_scalar:
-  forall cenv id s a f tf e le te sp lo hi m cs tm tv v m' fn k,
+  forall cenv id s a f tf e lenv te sp lo hi m cs tm tv v m' fn k,
   var_set_self cenv id s = OK a ->
-  match_callstack prog f m tm (Frame cenv tf e le te sp lo hi :: cs) (Mem.nextblock m) (Mem.nextblock tm) ->
+  match_callstack prog f m tm (Frame cenv tf e lenv te sp lo hi :: cs) (Mem.nextblock m) (Mem.nextblock tm) ->
   val_inject f v tv ->
   Mem.inject f m tm ->
   exec_assign ge e m id v m' ->
@@ -1281,7 +1313,7 @@ Lemma MS_var_set_self_correct_scalar:
     corestep_star CMin_core_sem tge (CMin_State fn a k (Vptr sp Int.zero) te) tm
                                     (CMin_State fn s k (Vptr sp Int.zero) te) tm' /\
     Mem.inject f m' tm' /\
-    match_callstack prog f m' tm' (Frame cenv tf e le te sp lo hi :: cs) (Mem.nextblock m') (Mem.nextblock tm') 
+    match_callstack prog f m' tm' (Frame cenv tf e lenv te sp lo hi :: cs) (Mem.nextblock m') (Mem.nextblock tm') 
 (********* The following 2 conditions are new*****)
    /\ (forall b, Mem.valid_block m b -> Mem.valid_block m' b) (* actually <-> holds*)
   /\ (forall b, Mem.valid_block tm b -> Mem.valid_block tm' b). (* actually <-> holds*)
@@ -1295,10 +1327,14 @@ Proof.
     inv MCS. inv MENV. auto.
   assert (EVAR: eval_expr tge (Vptr sp Int.zero) te tm (Evar (for_var id)) tv).
     constructor. auto.
-  revert VS; inv MV; intro VS; inv VS; inv H; try congruence.
+  revert VS; inv MV; intro VS; inv VS; inv H (*; try congruence. *).
+         Focus 2. rewrite H3 in H8; inv H8. 
+         Focus 3.  rewrite H3 in H5; inv H5.
+         Focus 3.  rewrite H3 in H5; inv H5.
+         Focus 3.  rewrite H3 in H5; inv H5.
   (* var_local *)
-  assert (b0 = b) by congruence. subst b0.
-  assert (chunk0 = chunk) by congruence. subst chunk0.
+  rewrite H3 in H8; inv H8. (*assert (b0 = b) by congruence. subst b0. 
+  assert (chunk0 = chunk) by congruence. subst chunk0.*)
   exists tm.
   split. apply corestep_star_zero. 
   split. eapply Mem.store_unmapped_inject; eauto. 
@@ -1307,7 +1343,7 @@ Proof.
     apply match_callstack_extensional with (PTree.set (for_var id) tv te).
     intros. repeat rewrite PTree.gsspec.
     destruct (peq (for_var id0) (for_var id)). congruence. auto.
-    intros. rewrite PTree.gso; auto. unfold for_temp, for_var; congruence.
+    intros. rewrite PTree.gso; auto. unfold for_temp, for_var. intros N. inv N. (* congruence.*)
     eapply match_callstack_store_local; eauto.
   split; intros; trivial. 
     (*apply prop_ext.
@@ -1341,9 +1377,9 @@ Proof.
 Qed.
 
 Lemma MS_var_set_self_correct_array:
-  forall cenv id s a f tf e le te sp lo hi m cs tm tv b v sz al m' fn k,
+  forall cenv id s a f tf e lenv te sp lo hi m cs tm tv b v sz al m' fn k,
   var_set_self cenv id s = OK a ->
-  match_callstack prog f m tm (Frame cenv tf e le te sp lo hi :: cs) (Mem.nextblock m) (Mem.nextblock tm) ->
+  match_callstack prog f m tm (Frame cenv tf e lenv te sp lo hi :: cs) (Mem.nextblock m) (Mem.nextblock tm) ->
   val_inject f v tv ->
   Mem.inject f m tm ->
   PTree.get id e = Some(b, Varray sz al) ->
@@ -1354,7 +1390,7 @@ Lemma MS_var_set_self_correct_array:
     corestep_star CMin_core_sem tge (CMin_State fn a k (Vptr sp Int.zero) te) tm
                                     (CMin_State fn s k (Vptr sp Int.zero) te) tm' /\
     Mem.inject f' m' tm' /\
-    match_callstack prog f' m' tm' (Frame cenv tf e le te sp lo hi :: cs) (Mem.nextblock m') (Mem.nextblock tm') /\
+    match_callstack prog f' m' tm' (Frame cenv tf e lenv te sp lo hi :: cs) (Mem.nextblock m') (Mem.nextblock tm') /\
     inject_incr f f'  /\
 (******* The following five conditions are new -- but actually, only conditions 3-5 or used below*****)
     Events.mem_unchanged_on (Events.loc_unmapped f) m m' /\
@@ -1481,19 +1517,19 @@ Proof. intros. inv MemCPY.
 Qed.
 
 Lemma MS_store_parameters_correct:
-  forall e le te m1 params vl m2,
+  forall e lenv te m1 params vl m2,
   bind_parameters ge e m1 params vl m2 ->
   forall s j1 cenv tf sp lo hi cs tm1 fn' k,
   vars_vals_match j1 params vl te ->
   list_norepet (List.map variable_name params) ->
   Mem.inject j1 m1 tm1 ->
-  match_callstack prog j1 m1 tm1 (Frame cenv tf e le te sp lo hi :: cs) (Mem.nextblock m1) (Mem.nextblock tm1) ->
+  match_callstack prog j1 m1 tm1 (Frame cenv tf e lenv te sp lo hi :: cs) (Mem.nextblock m1) (Mem.nextblock tm1) ->
   store_parameters cenv params = OK s ->
  exists j2, exists tm2,
      corestep_star CMin_core_sem tge (CMin_State fn' s k (Vptr sp Int.zero) te) tm1
                  (CMin_State fn' Sskip k (Vptr sp Int.zero) te) tm2
   /\ Mem.inject j2 m2 tm2
-  /\ match_callstack prog j2 m2 tm2 (Frame cenv tf e le te sp lo hi :: cs) (Mem.nextblock m2) (Mem.nextblock tm2)
+  /\ match_callstack prog j2 m2 tm2 (Frame cenv tf e lenv te sp lo hi :: cs) (Mem.nextblock m2) (Mem.nextblock tm2)
   /\ inject_incr j1 j2
 (********* The following 3 conditions are new*****)
   /\ Events.inject_separated j1 j2 m1 tm1
@@ -1630,7 +1666,7 @@ exists c2' : CMin_core,
 Proof. intros.
   generalize EQ; clear EQ; unfold transl_function.
   caseEq (build_compilenv gce f). intros ce sz BC.
-  destruct (zle sz Int.max_unsigned); try congruence.
+  destruct (zlenv sz Int.max_unsigned); try congruence.
   intro TRBODY.
   generalize TRBODY; intro TMP. monadInv TMP.
   set (tf := mkfunction (Csharpminor.fn_sig f) 
@@ -1665,23 +1701,1046 @@ Qed.
 (************************************************************************************)
 
 Lemma MS_step_case_Return:
-forall j m tm cs f e le k tk ty cenv v tv optid
+forall j m tm cs f e lenv k tk ty cenv v tv optid
 (MINJ : Mem.inject j m tm)
 (MCS : match_callstack prog j m tm cs (Mem.nextblock m) (Mem.nextblock tm))
-(MK : match_cont (Csharpminor.Kcall optid f e le k) tk ty cenv nil cs)
+(MK : match_cont (Csharpminor.Kcall optid f e lenv k) tk ty cenv nil cs)
 (RESINJ : val_inject j v tv),
 exists c2' : CMin_core,
   exists m2' : mem,
        corestep_plus CMin_core_sem tge (CMin_Returnstate tv tk) tm c2' m2'  /\
     exists c', 
        inj_match_states_star unit match_cores MC_measure (tt,c') j
-             (CSharpMin_State f Csharpminor.Sskip k e (set_optvar optid v le)) m c2' m2' .
+             (CSharpMin_State f Csharpminor.Sskip k e (set_optvar optid v lenv)) m c2' m2' .
 Proof. intros.
   inv MK. simpl.
   eexists; eexists; split.
        eapply corestep_plus_one. eapply CompCertStep_CMin_corestep'. econstructor; eauto. reflexivity.
   simpl.
-  exists  (CSharpMin_State f Csharpminor.Sskip k e (set_optvar optid v le)).
+  exists  (CSharpMin_State f Csharpminor.Sskip k e (set_optvar optid v lenv)).
+    left. unfold set_optvar. destruct optid; simpl option_map; econstructor; eauto.              
+         eapply match_callstack_set_temp; eauto. 
+Qed. 
+
+Lemma MS_step: forall (c1 : core_data) (m1 : mem) (c1' : core_data) (m1' : mem),
+corestep CSharpMin_CompcertCoreSem ge c1 m1 c1' m1' ->
+forall (c2 : CMin_core) (m2 : mem) (j : meminj),
+match_cores c1 j c1 m1 c2 m2 ->
+(exists c2' : CMin_core,
+   exists m2' : mem,
+     exists j' : meminj,
+       inject_incr j j' /\
+       Events.inject_separated j j' m1 m2 /\
+       corestep_plus CMin_CompcertCoreSem tge c2 m2 c2' m2' /\
+       match_cores c1' j' c1' m1' c2' m2') \/
+(MC_measure c1' < MC_measure c1)%nat /\ match_cores c1' j c1' m1' c2 m2.
+Proof.
+  intros. unfold core_data in *.
+   destruct (CSharpMin_corestep_2_CompCertStep _ _ _ _ _ H) as [t Ht]. simpl in *.
+  apply CSharpMin_corestep_not_at_external in H.
+   apply MC_MSI in H0. rename H0 into MSTATE.
+   inv Ht; simpl in *.
+  (*skip seq*)
+      destruct c1; simpl in *; try inv H1. 
+      destruct c1'; simpl in *; try inv H3.
+      inv MSTATE; simpl in *. 
+      monadInv TR.
+      destruct c2; simpl in *; try inv H8. 
+      destruct (MS_step_case_SkipSeq _ _ _ _ _ _ _ _ _ _ _ _ _ _ _ _ _ _ TRF MINJ MK MCS) as [c2' [m2' [cstepPlus MS]]].
+      left. exists c2'. exists m2'. exists j.
+      split. apply inject_incr_refl.
+      split. apply inject_separated_same_meminj.
+      auto.
+  (*skip Block*)
+      destruct c1; simpl in *; try inv H1. 
+      destruct c1'; simpl in *; try inv H3. 
+      inv MSTATE; simpl in *. 
+      monadInv TR.
+      destruct c2; simpl in *; try inv H8. 
+      destruct (MS_step_case_SkipBlock _ _ _ _ _ _ _ _ _ _ _ _ _ _ _ _ _ TRF MINJ MK MCS) as [c2' [m2' [cstepPlus MS]]].
+      left. exists c2'. exists m2'. exists j.
+      split. apply inject_incr_refl.
+      split. apply inject_separated_same_meminj.
+      auto.
+  (*skip Call*)
+      destruct c1; simpl in *; try inv H0. 
+      destruct c1'; simpl in *; try inv H1. 
+      inv MSTATE; simpl in *. 
+      monadInv TR.
+      destruct c2; simpl in *; try inv H11.
+      destruct (MS_step_case_SkipCall  _ _ _ _ _ _ _ _ _ _ _ _ _ _ _ _ _ _ H2 H3 H5 TRF MINJ MK MCS) as [c2' [m2' [cstepPlus MS]]].
+      left. exists c2'. exists m2'. exists j.
+      split. apply inject_incr_refl.
+      split. apply inject_separated_same_meminj.
+      auto.
+   (*assign*)
+      destruct c1; simpl in *; try inv H0. 
+      destruct c1'; simpl in *; try inv H1. 
+      inv MSTATE; simpl in *.
+      monadInv TR.
+      destruct c2; simpl in *; try inv H10.
+      rename  m1' into m'. rename m1 into m. rename m2 into tm. rename k0 into tk. rename f0 into tfn. rename e0 into te.
+      destruct (MS_step_case_Assign  _ _ _ _ _ _ _ _ _ _ _ _ _ _ _ _ _ _ _ _ _ _ _ _ H2 H4 TRF MINJ MK MCS EQ EQ0) as [c2' [m2' [cstepPlus MS]]].
+      left. exists c2'. exists m2'. exists j.
+      split. apply inject_incr_refl.
+      split. apply inject_separated_same_meminj.
+      auto.
+   (*set*)
+      destruct c1; simpl in *; try inv H0. 
+      destruct c1'; simpl in *; try inv H1. 
+      inv MSTATE; simpl in *.
+      monadInv TR.
+      destruct c2; simpl in *; try inv H9.
+      destruct (MS_step_case_Set _ _ _ _ _ _ _ _ _ _ _ _ _ _ _ _ _ _ _ _ _ id H3 TRF MINJ MCS MK EQ) as [c2' [m2' [cstepPlus MS]]].
+      left. exists c2'. exists m2'. exists j.
+      split. apply inject_incr_refl.
+      split. apply inject_separated_same_meminj.
+      auto.
+   (*store*)
+      destruct c1; simpl in *; try inv H0. 
+      destruct c1'; simpl in *; try inv H1. 
+      inv MSTATE; simpl in *.
+      monadInv TR.
+      destruct c2; simpl in *; try inv H11. rename f0 into tfn. rename m1 into m. rename m2  into tm. rename e0 into te. rename k0 into tk. rename  m1' into m'.
+      destruct (MS_step_case_Store _ _ _ _ _ _ _ _ _ _ _ _ _ _ _ _ _ _ _ _ _ _ _ _ _ _ _ H5 H2 H3 TRF MINJ MCS MK EQ EQ1) as [c2' [m2' [cstepPlus MS]]].
+      left. exists c2'. exists m2'. exists j.
+      split. apply inject_incr_refl.
+      split. apply inject_separated_same_meminj.
+      auto.
+   (*call*)
+      destruct c1; simpl in *; try inv H0. 
+      destruct c1'; simpl in *; try inv H1. 
+      inv MSTATE; simpl in *.
+      monadInv TR.
+      destruct c2; simpl in *; try inv H11. 
+      rename f into fd. rename f0 into f. rename f1 into tfn.
+      rename m1' into m. rename m2  into tm. rename e into te.
+      rename e0 into e.  rename k0 into tk. rename  le0 into le.
+      destruct (MS_step_case_Call _ _ _ _ _ _ _ _ _ _ _ _ _ _ _ _ _ _ _ _ _ _ _ optid _ _ H2 H3 H4 TRF MINJ MCS MK EQ EQ1) as [c2' [m2' [cstepPlusMS]]].
+      left. exists c2'. exists m2'. exists j.
+      split. apply inject_incr_refl.
+      split. apply inject_separated_same_meminj.
+      auto.
+  (*builtin*)
+      destruct c1; simpl in *; try inv H0. 
+      destruct c1'; simpl in *; try inv H1.
+      inv MSTATE; simpl in *. 
+      monadInv TR.
+      destruct c2; simpl in *; try inv H10.
+      rename f0 into tfn. 
+      rename m1 into m. rename m2  into tm. rename e into te.
+      rename e0 into e.  rename k0 into tk. rename  le0 into le.  rename m1' into m'.
+      destruct (MS_step_case_Builtin _ _ _ _ _ _ _ _ _ _ _ _ _ _ _ _ _ _ _ _ optid _ _ _ _ H2 H4 TRF MINJ MCS MK EQ) as [c2' [m2' [cstepPlus [j' [InjIncr [InjSep MS]]]]]].
+      left. exists c2'. exists m2'.  exists j'. auto.
+  (* seq *)
+      destruct c1; simpl in *; try inv H1. 
+      destruct c1'; simpl in *; try inv H3. 
+     rename k0 into k.
+      inv MSTATE. 
+      (*Case 1*) 
+         monadInv TR. left.
+         destruct c2; simpl in *; try inv H8.
+         rename f0 into tfn. rename e0 into te. rename k0 into tk.
+         exists  (CMin_State tfn x (Kseq x0 tk) (Vptr sp Int.zero) te). exists m2. 
+         exists j. 
+                split. apply inject_incr_refl.
+                split. apply inject_separated_same_meminj.
+                split; simpl.
+                    eapply corestep_plus_one.  eapply CompCertStep_CMin_corestep.  econstructor; eauto. reflexivity. 
+                econstructor; eauto.
+                          econstructor; eauto.
+      (* seq 2 *) 
+         destruct c2; simpl in *; try inv H9.
+         right. split. omega.
+                   econstructor; eauto.
+(* ifthenelse *)
+      destruct c1; simpl in *; try inv H0. 
+      destruct c1'; simpl in *; try inv H1. 
+      inv MSTATE. 
+      monadInv TR.
+      destruct c2; simpl in *; try inv H10. 
+         rename f0 into tfn. rename e0 into te. rename k0 into tk.
+      rename m1' into m. rename m2  into tm. 
+      destruct (MS_step_case_Ite _ _ _ _ _ _ _ _ _ _ _ _ _ _ _ _ _ _ _ _ _ _ _ _ _ _ H2 H4 TRF MINJ MCS MK EQ EQ1 EQ0) as [c2' [m2' [cstepPlus MS]]].
+      left. exists c2'. exists m2'. exists j.
+      split. apply inject_incr_refl.
+      split. apply inject_separated_same_meminj.
+      auto.
+  (*loop*)
+      destruct c1; simpl in *; try inv H1. 
+      destruct c1'; simpl in *; try inv H3. 
+      inv MSTATE. 
+      monadInv TR.
+      destruct c2; simpl in *; try inv H8. 
+         rename f0 into tfn. rename e0 into te. rename k0 into tk.
+      rename m1' into m. rename m2  into tm. 
+      destruct (MS_step_case_Loop _ _ _ _ _ _ _ _ _ _ _ _ _ _ _ _ _ _ _ TRF MINJ MCS MK EQ) as [c2' [m2' [cstepPlus MS]]].
+      left. exists c2'. exists m2'. exists j.
+      split. apply inject_incr_refl.
+      split. apply inject_separated_same_meminj.
+      auto.
+  (*block*)
+      destruct c1; simpl in *; try inv H1. 
+      destruct c1'; simpl in *; try inv H3. 
+      inv MSTATE. 
+      monadInv TR.
+      destruct c2; simpl in *; try inv H8. 
+         rename f0 into tfn. rename e0 into te. rename k0 into tk.
+      rename m1' into m. rename m2  into tm.  rename s0 into s.
+      destruct (MS_step_case_Block _ _ _ _ _ _ _ _ _ _ _ _ _ _ _ _ _ _ _ TRF MINJ MCS MK EQ) as [c2' [m2' [cstepPlus MS]]].
+      left. exists c2'. exists m2'. exists j.
+      split. apply inject_incr_refl.
+      split. apply inject_separated_same_meminj.
+      auto.
+  (*exit seq*)
+      destruct c1; simpl in *; try inv H1. 
+      destruct c1'; simpl in *; try inv H3. 
+      inv MSTATE. 
+      monadInv TR.
+      destruct c2; simpl in *; try inv H8. 
+         rename f0 into tfn. rename e0 into te. rename k0 into tk.
+      rename m1' into m. rename m2  into tm.
+      destruct (MS_step_case_ExitSeq _ _ _ _ _ _ _ _ _ _ _ _ _ _ _ _ _ n _ TRF MINJ MCS MK) as [c2' [m2' [cstepPlus MS]]].
+      left. exists c2'. exists m2'. exists j.
+      split. apply inject_incr_refl.
+      split. apply inject_separated_same_meminj.
+      auto.
+  (*exit block 0*)
+      destruct c1; simpl in *; try inv H1. 
+      destruct c1'; simpl in *; try inv H3. 
+      inv MSTATE. 
+      monadInv TR.
+      destruct c2; simpl in *; try inv H8. 
+         rename f0 into tfn. rename e0 into te. rename k0 into tk.
+      rename m1' into m. rename m2  into tm.
+      destruct (MS_step_case_ExitBlockZero _ _ _ _ _ _ _ _ _ _ _ _ _ _ _ _ _ TRF MINJ MCS MK) as [c2' [m2' [cstepPlus MS]]].
+      left. exists c2'. exists m2'. exists j.
+      split. apply inject_incr_refl.
+      split. apply inject_separated_same_meminj.
+      auto.
+  (*exit block n+1*)
+      destruct c1; simpl in *; try inv H1. 
+      destruct c1'; simpl in *; try inv H3. 
+      inv MSTATE. 
+      monadInv TR.
+      destruct c2; simpl in *; try inv H8. 
+         rename f0 into tfn. rename e0 into te. rename k0 into tk.
+      rename m1' into m. rename m2  into tm.
+      destruct (MS_step_case_ExitBlockNonzero _ _ _ _ _ _ _ _ _ _ _ _ _ _ _ _ _ n TRF MINJ MCS MK) as [c2' [m2' [cstepPlus MS]]].
+      left. exists c2'. exists m2'. exists j.
+      split. apply inject_incr_refl.
+      split. apply inject_separated_same_meminj.
+      auto.
+  (*switch*)
+      destruct c1; simpl in *; try inv H0. 
+      destruct c1'; simpl in *; try inv H1. 
+      inv MSTATE. 
+      monadInv TR.
+      destruct c2; simpl in *; try inv H9. 
+         rename f0 into tfn.  rename e0 into te.
+         rename k0 into tk. rename m1' into m. rename m2  into tm.  rename s into ts.
+      destruct (MS_step_case_Switch _ _ _ _ _ _ _ _ _ _ _ _ _ _ _ _ _ _ _ _ _ _ _ H3 TRF MINJ MCS MK EQ EQ0) as [c2' [m2' [cstepPlus MS]]].
+      left. exists c2'. exists m2'. exists j.
+      split. apply inject_incr_refl.
+      split. apply inject_separated_same_meminj.
+      auto.
+  (*return none*)
+      destruct c1; simpl in *; try inv H0. 
+      destruct c1'; simpl in *; try inv H1. 
+      inv MSTATE. 
+      monadInv TR.
+      destruct c2; simpl in *; try inv H9. 
+       rename f into tfn.  rename f0 into f. rename e into te. rename e0 into e.
+         rename k0 into tk. rename m1 into m. rename m2  into tm. rename m1'  into m'.  rename le0 into le.
+      destruct (MS_step_case_ReturnNone _ _ _ _ _ _ _ _ _ _ _ _ _ _ _ _ _ _ H3 TRF MINJ MCS MK) as [c2' [m2' [cstepPlus MS]]].
+      left. exists c2'. exists m2'. exists j.
+      split. apply inject_incr_refl.
+      split. apply inject_separated_same_meminj.
+      auto.
+  (*return some*)
+      destruct c1; simpl in *; try inv H0. 
+      destruct c1'; simpl in *; try inv H1. 
+      inv MSTATE. 
+      monadInv TR.
+      destruct c2; simpl in *; try inv H10. 
+       rename f into tfn.  rename f0 into f. rename e into te. rename e0 into e. rename k into tk.
+         rename k0 into k. rename m1 into m. rename m2  into tm. rename m1'  into m'.  rename le0 into le. rename v0 into v.
+      destruct (MS_step_case_ReturnSome _ _ _ _ _ _ _ _ _ _ _ _ _ _ _ _ _ _ _ _ _ _ H2 H4 TRF MINJ MCS MK EQ) as [c2' [m2' [cstepPlus MS]]].
+      left. exists c2'. exists m2'. exists j.
+      split. apply inject_incr_refl.
+      split. apply inject_separated_same_meminj.
+      auto.
+  (*label*)
+      destruct c1; simpl in *; try inv H1. 
+      destruct c1'; simpl in *; try inv H3. 
+      inv MSTATE. 
+      monadInv TR.
+      destruct c2; simpl in *; try inv H8. 
+       rename f0 into tfn. rename e0 into te. 
+         rename k0 into tk. rename m1' into m. rename m2  into tm. rename s0 into s.  
+      destruct (MS_step_case_Label _ _ _ _ _ _ _ _ _ _ _ _ _ _ _ _ _ lbl _ _ TRF MINJ MCS MK EQ) as [c2' [m2' [cstepPlus MS]]].
+      left. exists c2'. exists m2'. exists j.
+      split. apply inject_incr_refl.
+      split. apply inject_separated_same_meminj.
+      auto.
+  (*goto*)
+      destruct c1; simpl in *; try inv H0. 
+      destruct c1'; simpl in *; try inv H1. 
+      inv MSTATE. 
+      monadInv TR.
+      destruct c2; simpl in *; try inv H9. 
+       rename f0 into tfn. rename e0 into te. 
+         rename k1 into tk. rename s into s'.  rename k into k'. rename k0 into k. rename m1' into m. rename m2  into tm.
+      destruct (MS_step_case_Goto _ _ _ _ _ _ _ _ _ _ _ _ _ _ _ _ _ _ _ _ H3 TRF MINJ MCS MK) as [c2' [m2' [cstepPlus MS]]].
+      left. exists c2'. exists m2'. exists j.
+      split. apply inject_incr_refl.
+      split. apply inject_separated_same_meminj.
+      auto.
+(* internal call *)
+      destruct c1; simpl in *; try inv H0. 
+      destruct c1'; simpl in *; try inv H1. 
+      inv MSTATE. 
+      monadInv TR.
+      destruct c2; simpl in *; try inv H9. 
+      rename m1 into m. rename m2 into tm. rename f0 into f. rename e0 into e.
+      rename m0 into m1. rename args into vargs. rename m1' into m2.
+      rename k0 into tk. rename args0 into targs. 
+      destruct (MS_step_case_InternalCall _ _ _ _ _ _ _ _ _ _ _ _ _ _ H2 H3 H5 MINJ MCS MK ISCC ARGSINJ EQ) as [c2' [m2' [cstepPlus [j' [InjIncr [InjSep [c' MS]]]]]]].
+      exists c2'. exists m2'. exists (tt,c'). exists j'. auto.
+(* external call *)
+      destruct c1; simpl in *; try inv H0. inv H. 
+   (*nothing to show here - cf corestep not at external *) 
+ (*     destruct c1'; simpl in *; try inv H1. 
+      inv MSTATE. 
+      monadInv TR.
+      destruct c2; simpl in *; try inv H7.  
+      rename m1 into m. rename m2 into tm. 
+      rename k0 into tk. rename args0 into targs.  rename m1' into m'. 
+  inv MSTATE. monadInv TR. rename f into j.
+  destruct (transl_step_case_ExternalCall _ _ _ _ _ _ _ _ _ _ _ _ _ H MINJ MCS MK ISCC ARGSINJ) as [T2 [Steps [j' [Inc MSI]]]].
+   apply matchInj_Elim in MSI. eauto.*)
+
+(* return *)
+      destruct c1; simpl in *; try inv H1. 
+      destruct c1'; simpl in *; try inv H3. 
+      inv MSTATE. 
+      destruct c2; simpl in *; try inv H5. rename m1' into m. rename m2 into tm. rename f0 into f. rename e0 into e. rename k into tk. rename k0 into k. rename v into tv. rename v0 into v.
+      destruct (MS_step_case_Return _ _ _ _ _ _ _ _ _ _ _ _ tv optid MINJ MCS MK RESINJ) as [c2' [m2' [cstepPlus [c' MS]]]]. 
+      exists c2'. exists m2'. exists (tt,c'). exists j.
+      split. apply inject_incr_refl.
+      split. apply inject_separated_same_meminj.
+      auto. 
+Qed.
+Goal forall entrypoints, 
+Sim_inj.Forward_simulation_inject _ _ CSharpMin_CompcertCoreSem 
+   CMin_CompcertCoreSem ge tge entrypoints.
+Proof.
+intros. apply inj_simulation_star with (match_states:=match_cores)(measure:=MC_measure).
+   intros. eapply (init_cores _ _ _ entrypoints); eauto.
+   apply MC_safely_halted.
+   apply MC_at_external.
+   apply  MC_after_external.
+
+
+Goal forall entrypoints, 
+Sim_inj.Forward_simulation_inject _ _ CSharpMin_CompcertCoreSem 
+   CMin_CompcertCoreSem ge tge entrypoints.
+Proof.
+intros. apply inj_simulation_star with (match_states:=match_cores)(measure:=MC_measure).
+   intros. eapply (init_cores _ _ _ entrypoints); eauto.
+   apply MC_safely_halted.
+   apply MC_at_external.
+   apply  MC_after_external.
+Admitted.
+
+
+(******************************Functions required for internal call rule*****************************)
+(****These extend the original lemmas by additional guarantees of the (now exposed) memory injections, in order
+    for the overall lemma for internal calls to establish the inject_separated fact******************************)
+Lemma MS_match_callstack_alloc_variable:
+  forall atk id lv cenv sz cenv' sz' tm sp e tf m m' b te lenv lo cs f tv,
+  assign_variablenv atk (id, lv) (cenv, sz) = (cenv', sz') ->
+  Mem.valid_block tm sp ->
+  (forall ofs k p,
+    Mem.perm tm sp ofs k p -> 0 <= ofs < tf.(fn_stackspace)) ->
+  Mem.range_perm tm sp 0 tf.(fn_stackspace) Cur Freeablenv ->
+  tf.(fn_stackspace) <= Int.max_unsigned ->
+  Mem.alloc m 0 (sizeof lv) = (m', b) ->
+  match_callstack prog f m tm 
+                  (Frame cenv tf e lenv te sp lo (Mem.nextblock m) :: cs)
+                  (Mem.nextblock m) (Mem.nextblock tm) ->
+  Mem.inject f m tm ->
+  0 <= sz -> sz' <= tf.(fn_stackspace) ->
+  (forall b delta ofs k p,
+     f b = Some(sp, delta) -> Mem.perm m b ofs k p -> ofs + delta < sz) ->
+  e!id = None ->
+  te!(for_var id) = Some tv ->
+  exists f',
+     inject_incr f f'
+  /\ Mem.inject f' m' tm
+  /\ match_callstack prog f' m' tm
+                     (Frame cenv' tf (PTree.set id (b, lv) e) lenv te sp lo (Mem.nextblock m') :: cs)
+                     (Mem.nextblock m') (Mem.nextblock tm)
+  /\ (forall b delta ofs k p,
+      f' b = Some(sp, delta) -> Mem.perm m' b ofs k p -> ofs + delta < sz') 
+(****************The following three conditions are new******************)
+  /\ (forall b, Mem.valid_block m b -> f' b = f b)
+  /\ (forall b b' d', f b = None -> f' b = Some (b',d') -> b' = sp)
+  /\ forall j',  inject_incr f' j' -> Events.inject_separated f' j' m' tm -> Events.inject_separated f' j' m tm.
+Proof.
+  intros until tv. intros ASV VALID BOUNDS PERMS NOOV ALLOC MCS INJ LO HI RANGE E TE.
+  generalize ASV. unfold assign_variable. 
+  caseEq lv.
+  (* 1. lv = LVscalar chunk *)
+  intros chunk LV. case (Identset.mem id atk).
+  (* 1.1 info = Var_stack_scalar chunk ofs *)
+    set (ofs := align sz (size_chunk chunk)).
+    intro EQ; injection EQ; intros; clear EQ. rewrite <- H0.
+    generalize (size_chunk_pos chunk); intro SIZEPOS.
+    generalize (align_lenv sz (size_chunk chunk) SIZEPOS). fold ofs. intro SZOFS.
+    exploit Mem.alloc_left_mapped_inject.
+      eauto. eauto. eauto. 
+      instantiate (1 := ofs). omega.
+      intros. exploit BOUNDS; eauto. omega. 
+      intros. apply Mem.perm_implies with Freeable; auto with mem. apply Mem.perm_cur. 
+      apply PERMS. rewrite LV in H1. simpl in H1. omega.
+      rewrite LV; simpl. rewrite Zminus_0_r. unfold ofs. 
+      apply inj_offset_aligned_var.
+      intros. generalize (RANGE _ _ _ _ _ H1 H2). omega. 
+    intros [f1 [MINJ1 [INCR1 [SAME OTHER]]]].
+    exists f1; split. auto. split. auto. split. 
+    eapply match_callstack_alloc_left; eauto.
+    rewrite <- LV; auto. 
+    rewrite SAME; constructor.
+  split.
+    intros. exploit Mem.perm_alloc_inv; eauto. destruct (zeq b0 b).
+    subst b0. assert (delta = ofs) by congruence. subst delta.  
+    rewrite LV. simpl. omega.
+    intro. rewrite OTHER in H1; eauto. generalize (RANGE _ _ _ _ _ H1 H3). omega. 
+  assert (XX: forall b0 : Values.block, Mem.valid_block m b0 -> f1 b0 = f b0).
+     intros b0; intros. destruct (eq_block b0 b); subst. 
+                     exfalso. apply (Mem.fresh_block_alloc _ _ _ _ _ ALLOC H1).
+                  apply (OTHER _ n).
+   split; trivial.
+   split; intros. destruct (eq_block b0 b); subst. rewrite SAME in H2. inv H2. trivial.
+                         rewrite (OTHER _ n) in H2. congruence. 
+     intros. intros bb; intros.
+     destruct (H2 _ _ _ H3 H4). split; trivial. intros N. apply H5. eapply Mem.valid_block_alloc; eauto.
+  (* 1.2 info = Var_local chunk *)
+    intro EQ; injection EQ; intros; clear EQ. subst sz'. rewrite <- H0.
+    exploit Mem.alloc_left_unmapped_inject; eauto.
+    intros [f1 [MINJ1 [INCR1 [SAME OTHER]]]].
+    exists f1; split. auto. split. auto. split.
+      eapply match_callstack_alloc_left; eauto.  
+      rewrite <- LV; auto.
+      rewrite SAME; constructor.
+   split.
+      intros. exploit Mem.perm_alloc_inv; eauto. destruct (zeq b0 b).
+      subst b0. congruence.
+      rewrite OTHER in H; eauto.
+  assert (XX: forall b0 : Values.block, Mem.valid_block m b0 -> f1 b0 = f b0).
+     intros b0; intros. destruct (eq_block b0 b); subst. 
+                     exfalso. apply (Mem.fresh_block_alloc _ _ _ _ _ ALLOC H).
+                  apply (OTHER _ n).
+   split; trivial.
+   split; intros. destruct (eq_block b0 b); subst. rewrite SAME in H1. inv H1.
+                         rewrite (OTHER _ n) in H1. congruence. 
+   intros bb; intros.
+     destruct (H1 _ _ _ H2 H3). split; trivial. intros N. apply H4. eapply Mem.valid_block_alloc; eauto.
+  (* 2 info = Var_stack_array ofs *)
+  intros dim al LV EQ. injection EQ; clear EQ; intros. rewrite <- H.
+  assert (0 <= Zmax 0 dim). apply Zmax1. 
+  generalize (align_lenv sz (array_alignment dim) (array_alignment_pos dim)). intro.
+  set (ofs := align sz (array_alignment dim)) in *.
+  exploit Mem.alloc_left_mapped_inject. eauto. eauto. eauto. 
+    instantiate (1 := ofs). 
+    generalize Int.min_signed_neg. omega.
+    intros. exploit BOUNDS; eauto. generalize Int.min_signed_neg. omega.
+    intros. apply Mem.perm_implies with Freeable; auto with mem. apply Mem.perm_cur.
+    apply PERMS. rewrite LV in H3. simpl in H3. omega.
+    rewrite LV; simpl. rewrite Zminus_0_r. unfold ofs. 
+    apply inj_offset_aligned_array'.
+    intros. generalize (RANGE _ _ _ _ _ H3 H4). omega. 
+  intros [f1 [MINJ1 [INCR1 [SAME OTHER]]]].
+  exists f1; split. auto. split. auto. split. 
+    subst cenv'. eapply match_callstack_alloc_left; eauto.
+    rewrite <- LV; auto. 
+    rewrite SAME; constructor.
+  split.
+    intros. exploit Mem.perm_alloc_inv; eauto. destruct (zeq b0 b).
+    subst b0. assert (delta = ofs) by congruence. subst delta. 
+    rewrite LV. simpl. omega.
+    intro. rewrite OTHER in H3; eauto. generalize (RANGE _ _ _ _ _ H3 H5). omega. 
+  assert (XX: forall b0 : Values.block, Mem.valid_block m b0 -> f1 b0 = f b0).
+     intros b0; intros. destruct (eq_block b0 b); subst. 
+                     exfalso. apply (Mem.fresh_block_alloc _ _ _ _ _ ALLOC H3).
+                  apply (OTHER _ n).
+   split; trivial.
+   split; intros. destruct (eq_block b0 b); subst. rewrite SAME in H4. inv H4. trivial.
+                         rewrite (OTHER _ n) in H4. congruence. 
+   intros bb; intros.
+     destruct (H4 _ _ _ H5 H6). split; trivial. intros N. apply H7. eapply Mem.valid_block_alloc; eauto.
+Qed.
+
+Lemma MS_match_callstack_alloc_variables_rec:
+  forall tm sp cenv' tf lenv te lo cs atk,
+  Mem.valid_block tm sp ->
+  (forall ofs k p,
+    Mem.perm tm sp ofs k p -> 0 <= ofs < tf.(fn_stackspace)) ->
+  Mem.range_perm tm sp 0 tf.(fn_stackspace) Cur Freeablenv ->
+  tf.(fn_stackspace) <= Int.max_unsigned ->
+  forall e m vars e' m',
+  alloc_variables e m vars e' m' ->
+  forall f cenv sz,
+  assign_variables atk vars (cenv, sz) = (cenv', tf.(fn_stackspace)) ->
+  match_callstack prog f m tm 
+                  (Frame cenv tf e lenv te sp lo (Mem.nextblock m) :: cs)
+                  (Mem.nextblock m) (Mem.nextblock tm) ->
+  Mem.inject f m tm ->
+  0 <= sz ->
+  (forall b delta ofs k p,
+     f b = Some(sp, delta) -> Mem.perm m b ofs k p -> ofs + delta < sz) ->
+  (forall id lv, In (id, lv) vars -> te!(for_var id) <> None) ->
+  list_norepet (List.map (@fst ident var_kind) vars) ->
+  (forall id lv, In (id, lv) vars -> e!id = None) ->
+  exists f',
+     inject_incr f f'
+  /\ Mem.inject f' m' tm
+  /\ match_callstack prog f' m' tm
+                     (Frame cenv' tf e' lenv te sp lo (Mem.nextblock m') :: cs)
+                     (Mem.nextblock m') (Mem.nextblock tm)
+(****************The following three conditions are new******************)
+(*** Note that in the third clause, we only "step" from m' to m ***************)
+  /\ (forall b, Mem.valid_block m b -> f' b = f b)
+  /\ (forall b b' d', f b = None -> f' b = Some (b',d') -> b' = sp)
+  /\ forall j',  inject_incr f' j' -> Events.inject_separated f' j' m' tm -> Events.inject_separated f' j' m tm .
+Proof.
+  intros until atk. intros VALID BOUNDS PERM NOOV.
+  induction 1.
+  (* base case *)
+  intros. simpl in H. inversion H; subst cenv sz.
+  exists f. split. apply inject_incr_refl. split. auto. split. auto.
+    split; trivial.
+    split; trivial. intros. congruence.
+  (* inductive case *)
+  intros until sz.
+  change (assign_variables atk ((id, lv) :: vars) (cenv, sz))
+  with (assign_variables atk vars (assign_variablenv atk (id, lv) (cenv, sz))).
+  caseEq (assign_variablenv atk (id, lv) (cenv, sz)).
+  intros cenv1 sz1 ASV1 ASVS MATCH MINJ SZPOS BOUND DEFINED NOREPET UNDEFINED.
+  assert (DEFINED1: forall id0 lv0, In (id0, lv0) vars -> te!(for_var id0) <> None).
+    intros. eapply DEFINED. simpl. right. eauto.
+  assert (exists tv, te!(for_var id) = Some tv).
+    assert (te!(for_var id) <> None). eapply DEFINED. simpl; left; auto.
+    destruct (te!(for_var id)). exists v; auto. congruence.
+  destruct H1 as [tv TEID].
+  assert (sz1 <= fn_stackspace tf). eapply assign_variables_incr; eauto. 
+  exploit MS_match_callstack_alloc_variable; eauto with coqlib.
+  intros [f1 [INCR1 [INJ1 [MCS1 [BOUND1 [VB [SP SEP]]]]]]].
+  exploit IHalloc_variables; eauto. 
+  apply Zle_trans with sz; auto. eapply assign_variable_incr; eauto.
+  inv NOREPET; auto.
+  intros. rewrite PTree.gso. eapply UNDEFINED; eauto with coqlib.
+  simpl in NOREPET. inversion NOREPET. red; intro; subst id0.
+  elim H5. change id with (fst (id, lv0)). apply List.in_map. auto.
+  intros [f2 [INCR2 [INJ2 [MCS2 [VBF2 [SP2 SEP2]]]]]].
+  assert (X: forall b : Values.block, Mem.valid_block m b -> f2 b = f b).
+           intros. rewrite <- (VB _ H2). apply VBF2. eapply Mem.valid_block_alloc; eauto.
+  assert (Y:  (forall (b b' : Values.block) (d' : Z), f b = None -> f2 b = Some (b', d') -> b' = sp)).
+       clear MCS2 BOUND1 MCS1 DEFINED1 SEP SEP2 IHalloc_variables UNDEFINED.
+          intros. remember (f1 b) as z. destruct z; apply eq_sym in Heqz.
+              destruct p.  assert (Z1 := SP _ _ _ H2 Heqz). subst.
+                 apply INCR2 in Heqz. rewrite Heqz in H3. inv H3. trivial.
+             apply (SP2 _ _ _ Heqz H3).
+  exists f2 ; intuition.
+    eapply inject_incr_trans; eauto.
+    intros b; intros. destruct (H3 _ _ _ H4 H5). split; trivial.
+     intros N. apply H6. apply (Mem.valid_block_alloc _ _ _ _ _ H) in N.
+              eapply allocvars_blocks_valid; eauto.
+Qed. 
+
+Lemma MS_match_callstack_alloc_variables:
+  forall fn cenv tf m e m' tm tm' sp f cs targs,
+  build_compilenv gce fn = (cenv, tf.(fn_stackspace)) ->
+  tf.(fn_stackspace) <= Int.max_unsigned ->
+  list_norepet (fn_params_names fn ++ fn_vars_names fn) ->
+  alloc_variables Csharpminor.empty_env m (fn_variables fn) e m' ->
+  Mem.alloc tm 0 tf.(fn_stackspace) = (tm', sp) ->
+  match_callstack prog f m tm cs (Mem.nextblock m) (Mem.nextblock tm) ->
+  Mem.inject f m tm ->
+  let tparams := List.map for_var (fn_params_names fn) in
+  let tvars := List.map for_var (fn_vars_names fn) in
+  let ttemps := List.map for_temp (Csharpminor.fn_temps fn) in
+  let te := set_locals (tvars ++ ttemps) (set_params targs tparams) in
+  exists f',
+     inject_incr f f'
+  /\ Mem.inject f' m' tm'
+  /\ match_callstack prog f' m' tm'
+                     (Frame cenv tf e empty_temp_env te sp (Mem.nextblock m) (Mem.nextblock m') :: cs)
+                     (Mem.nextblock m') (Mem.nextblock tm') 
+(****************The following three conditions are new******************)
+(* In the third clause, we now stepfrom  m' to m, and also from f' to f and from tm' to tm******************)
+  /\ (forall b, Mem.valid_block m b -> f' b = f b)
+  /\ (forall b b' d', f b = None -> f' b = Some (b',d') -> b' = sp)
+  /\ forall j',  inject_incr f' j' -> Events.inject_separated f' j' m' tm' -> Events.inject_separated f j' m tm.
+Proof.
+  intros.
+  unfold build_compilenv in H.
+assert (AR: exists f',
+     inject_incr f f'
+  /\ Mem.inject f' m' tm'
+  /\ match_callstack prog f' m' tm'
+                     (Frame cenv tf e empty_temp_env te sp (Mem.nextblock m) (Mem.nextblock m') :: cs)
+                     (Mem.nextblock m') (Mem.nextblock tm') 
+  /\ (forall b, Mem.valid_block m b -> f' b = f b)
+  /\ (forall b b' d', f b = None -> f' b = Some (b',d') -> b' = sp)
+  /\ forall j',  inject_incr f' j' -> Events.inject_separated f' j' m' tm' -> Events.inject_separated f' j' m tm').
+  eapply MS_match_callstack_alloc_variables_rec; eauto with mem.
+  red; intros. eapply Mem.perm_alloc_2; eauto. 
+  eapply match_callstack_alloc_right; eauto.
+  eapply Mem.alloc_right_inject; eauto. omega. 
+  intros. elim (Mem.valid_not_valid_diff tm sp sp); eauto with mem.
+  eapply Mem.valid_block_inject_2; eauto.
+  intros. unfold te. apply set_locals_params_defined.
+  elim (in_app_or _ _ _ H6); intros.
+  apply in_or_app; left. unfold tparams. apply List.in_map.
+  change id with (fst (id, lv)). apply List.in_map. auto.
+  apply in_or_app; right. apply in_or_app; left. unfold tvars. apply List.in_map. 
+  change id with (fst (id, lv)). apply List.in_map; auto.
+  (* norepet *)
+  unfold fn_variables. rewrite List.map_app. assumption.
+  (* undef *)
+  intros. unfold empty_env. apply PTree.gempty.
+
+destruct AR as  [f' [INC [INJ [MC [VB1 [SP SEP]]]]]].
+exists f' ; intuition.
+  intros b; intros.
+  remember (f' b) as z; destruct z; apply eq_sym in Heqz.
+  (*Some p*) destruct p.
+            assert (j' b = Some (b0,z)). apply (H6 _ _ _ Heqz). 
+             rewrite H9 in H10; inv H10.
+             assert (Z:= SP _ _ _ H8 Heqz); subst.
+             split; intros N. rewrite (VB1 _ N) in Heqz. congruence.
+             eapply (Mem.fresh_block_alloc _ _ _ _ _ H3 N).
+  (*None*) assert (HH:= SEP _ H6 H7).
+                     destruct (HH _ _ _ Heqz H9).
+                     split; trivial. 
+                     intros N. apply H11. eapply Mem.valid_block_alloc; eauto. 
+Qed.
+
+Lemma MS_var_set_self_correct_scalar:
+  forall cenv id s a f tf e lenv te sp lo hi m cs tm tv v m' fn k,
+  var_set_self cenv id s = OK a ->
+  match_callstack prog f m tm (Frame cenv tf e lenv te sp lo hi :: cs) (Mem.nextblock m) (Mem.nextblock tm) ->
+  val_inject f v tv ->
+  Mem.inject f m tm ->
+  exec_assign ge e m id v m' ->
+  te!(for_var id) = Some tv ->
+  exists tm',
+    corestep_star CMin_core_sem tge (CMin_State fn a k (Vptr sp Int.zero) te) tm
+                                    (CMin_State fn s k (Vptr sp Int.zero) te) tm' /\
+    Mem.inject f m' tm' /\
+    match_callstack prog f m' tm' (Frame cenv tf e lenv te sp lo hi :: cs) (Mem.nextblock m') (Mem.nextblock tm') 
+(********* The following 2 conditions are new*****)
+   /\ (forall b, Mem.valid_block m b -> Mem.valid_block m' b) (* actually <-> holds*)
+  /\ (forall b, Mem.valid_block tm b -> Mem.valid_block tm' b). (* actually <-> holds*)
+Proof.
+  intros until k. 
+  intros VS MCS VINJ MINJ ASG VAL.
+  unfold var_set_self in VS. inv ASG. 
+  assert (NEXTBLOCK: Mem.nextblock m' = Mem.nextblock m).
+    eapply Mem.nextblock_store; eauto.
+  assert (MV: match_var prog f id e m te sp cenv!!id).
+    inv MCS. inv MENV. auto.
+  assert (EVAR: eval_expr tge (Vptr sp Int.zero) te tm (Evar (for_var id)) tv).
+    constructor. auto.
+  revert VS; inv MV; intro VS; inv VS; inv H; try congruence.
+  (* var_local *)
+  assert (b0 = b) by congruence. subst b0.
+  assert (chunk0 = chunk) by congruence. subst chunk0.
+  exists tm.
+  split. apply corestep_star_zero. 
+  split. eapply Mem.store_unmapped_inject; eauto. 
+  rewrite NEXTBLOCK. 
+  split.
+    apply match_callstack_extensional with (PTree.set (for_var id) tv te).
+    intros. repeat rewrite PTree.gsspec.
+    destruct (peq (for_var id0) (for_var id)). congruence. auto.
+    intros. rewrite PTree.gso; auto. unfold for_temp, for_var; congruence.
+    eapply match_callstack_store_local; eauto.
+  split; intros; trivial. 
+    (*apply prop_ext.
+    split; intros. *) eapply Mem.store_valid_block_1; eauto.
+     (* eapply Mem.store_valid_block_2; eauto.*)
+  (* var_stack_scalar *)
+  assert (b0 = b) by congruence. subst b0.
+  assert (chunk0 = chunk) by congruence. subst chunk0.
+  assert (Mem.storev chunk m (Vptr b Int.zero) v = Some m'). assumption.
+  exploit make_store_correct.
+    eapply make_stackaddr_correct.
+    eauto. eauto. eauto. eauto. eauto. 
+  intros [tm' [tvrhs' [EVAL' [STORE' MEMINJ]]]].
+  exists tm'.
+  split. eapply corestep_star_trans.
+           eapply corestep_star_one. eapply CompCertStep_CMin_corestep'. econstructor. reflexivity.
+         simpl. 
+         eapply corestep_star_trans.
+           eapply corestep_star_one. eapply CompCertStep_CMin_corestep'. apply EVAL'. reflexivity. 
+         simpl.
+           eapply corestep_star_one. eapply CompCertStep_CMin_corestep. constructor. reflexivity.
+  split. trivial.
+  split.
+    rewrite NEXTBLOCK. rewrite (nextblock_storev _ _ _ _ _ STORE'). 
+    eapply match_callstack_storev_mapped; eauto.
+  split; intros. 
+    (*apply prop_ext; split; intros. *) eapply Mem.store_valid_block_1; eauto.
+           (* eapply Mem.store_valid_block_2; eauto.  *)
+    inv EVAL'.  (*apply prop_ext; split; intros.  *) eapply storev_valid_block_1; eauto.
+                             (*eapply storev_valid_block_2; eauto.   *)
+Qed.
+
+Lemma MS_var_set_self_correct_array:
+  forall cenv id s a f tf e lenv te sp lo hi m cs tm tv b v sz al m' fn k,
+  var_set_self cenv id s = OK a ->
+  match_callstack prog f m tm (Frame cenv tf e lenv te sp lo hi :: cs) (Mem.nextblock m) (Mem.nextblock tm) ->
+  val_inject f v tv ->
+  Mem.inject f m tm ->
+  PTree.get id e = Some(b, Varray sz al) ->
+  Events.extcall_memcpy_sem sz (Zmin al 4) ge
+                             (Vptr b Int.zero :: v :: nil) m Events.E0 Vundef m' ->
+  te!(for_var id) = Some tv ->
+  exists f', exists tm',
+    corestep_star CMin_core_sem tge (CMin_State fn a k (Vptr sp Int.zero) te) tm
+                                    (CMin_State fn s k (Vptr sp Int.zero) te) tm' /\
+    Mem.inject f' m' tm' /\
+    match_callstack prog f' m' tm' (Frame cenv tf e lenv te sp lo hi :: cs) (Mem.nextblock m') (Mem.nextblock tm') /\
+    inject_incr f f'  /\
+(******* The following five conditions are new -- but actually, only conditions 3-5 or used below*****)
+    Events.mem_unchanged_on (Events.loc_unmapped f) m m' /\
+    Events.mem_unchanged_on (Events.loc_out_of_reach f m) tm tm' /\
+    Events.inject_separated f f' m tm  /\
+    (forall b, Mem.valid_block m b -> Mem.valid_block m' b) (* actually <-> holds*)
+  /\ (forall b, Mem.valid_block tm b -> Mem.valid_block tm' b). 
+Proof.
+  intros until k. 
+  intros VS MCS VINJ MINJ KIND MEMCPY VAL.
+  assert (MV: match_var prog f id e m te sp cenv!!id).
+    inv MCS. inv MENV. auto.
+  inv MV; try congruence. rewrite KIND in H0; inv H0.
+  (* var_stack_array *)
+  unfold var_set_self in VS. rewrite <- H in VS. inv VS.
+  exploit match_callstack_match_globalenvs; eauto. intros [hi' MG].
+  assert (Events.external_call (EF_memcpy sz0 (Zmin al0 4)) ge (Vptr b0 Int.zero :: v :: nil) m Events.E0 Vundef m').
+    assumption.
+  exploit Events.external_call_mem_inject; eauto. 
+  eapply inj_preserves_globals; eauto.
+  intros [f' [vres' [tm' [EC' [VINJ' [MINJ' [UNMAPPED [OUTOFREACH [INCR SEPARATED]]]]]]]]].
+  exists f'; exists tm'.
+  split. eapply corestep_star_trans.
+           eapply corestep_star_one. eapply CompCertStep_CMin_corestep'. constructor. reflexivity. 
+         simpl.
+         eapply corestep_star_trans.
+           eapply corestep_star_one. eapply CompCertStep_CMin_corestep'. econstructor; eauto. 
+                constructor. apply make_stackaddr_correct. constructor. constructor. eauto. constructor.
+                  eapply Events.external_call_symbols_preserved_2; eauto.
+                  apply symbols_preserved. assumption.
+                  apply var_info_translated. assumption.
+                  apply var_info_rev_translated. assumption.
+               reflexivity.
+         simpl. eapply corestep_star_one. eapply CompCertStep_CMin_corestep. constructor. reflexivity.
+  split. auto.
+  split. apply match_callstack_incr_bound with (Mem.nextblock m) (Mem.nextblock tm).
+  eapply match_callstack_external_call; eauto.
+  intros. eapply Events.external_call_max_perm; eauto.
+  omega. omega.
+  eapply external_call_nextblock_incr; eauto.
+  eapply external_call_nextblock_incr; eauto.
+split.  auto.
+split; trivial.
+split; trivial.
+split; trivial.
+split; intros. inv MEMCPY. eapply Mem.storebytes_valid_block_1; eauto.
+   (*    apply prop_ext; split; intros. eapply Mem.storebytes_valid_block_1; eauto. eapply Mem.storebytes_valid_block_2; eauto.      *)
+eapply Events.external_call_valid_block; eauto. 
+Qed.
+
+(*Lemma appears to be new*)
+Lemma bind_parameters_validblock_2:
+forall gee e params vals m1 m2 (BP: bind_parameters gee e m1 params vals m2)
+b (B1:Mem.valid_block m2 b), Mem.valid_block m1 b.
+Proof. intros gee e params.
+  induction params; intros.
+   inv BP. trivial.
+  destruct vals; inv BP.
+    (*skalar*)
+      eapply Mem.store_valid_block_2. apply H8.
+      eapply (IHparams _ _ _ H9 _ B1). 
+    (*array*)
+      inv H7.
+      eapply Mem.storebytes_valid_block_2. apply H13.
+      eapply (IHparams _ _ _ H8 _ B1). 
+Qed.
+
+(*Lemma appears to be new, but was not needed after all in new proof*)
+Lemma bind_parameters_validblock_1:
+forall gee e params vals m1 m2 (BP: bind_parameters gee e m1 params vals m2)
+b (B1:Mem.valid_block m1 b), Mem.valid_block m2 b.
+Proof. intros gee e params.
+  induction params; intros.
+   inv BP. trivial.
+  destruct vals; inv BP.
+    (*skalar*)
+      eapply (IHparams _ _ _ H9). clear IHparams H9.
+      eapply Mem.store_valid_block_1; eauto.
+    (*array*)
+      eapply (IHparams _ _ _ H8). clear IHparams H8.
+      inv H7. 
+      eapply Mem.storebytes_valid_block_1; eauto.
+Qed.
+
+(*Lemma appears to be new, but was not needed after all in new proof*)
+Lemma bind_parameters_inject_separated_skalar:
+forall gee e params vals m1 m2 f' tm3 j tm1 m tm2 v b ch
+(CH: Mem.store ch m b 0 v = Some m1)
+(BP: bind_parameters gee e m1 params vals m2)
+(MINJ : Mem.inject f' m2 tm3)
+(SEP : Events.inject_separated j f' m1 tm2),
+Events.inject_separated j f' m tm1.
+Proof. intros.
+  intros bb; intros.
+     unfold Events.inject_separated in SEP.
+     destruct (SEP _ _ _ H H0).
+     split; intros XX.  
+       apply H1. eapply Mem.store_valid_block_1; eauto.
+     assert (~ Mem.valid_block m2 bb).
+       intros ZZ. apply H1. apply (bind_parameters_validblock_2 _ _ _ _ _ _ BP _ ZZ). 
+       unfold Mem.inject in MINJ. destruct MINJ.
+         rewrite (mi_freeblocks _ H3) in H0. inv H0.    
+Qed.
+
+(*Lemma appears to be new, but was not needed after all in new proof*)
+Lemma bind_parameters_inject_separated_array:
+forall gee e params vals m1 m2  m cpvals t n sz
+(MemCPY: Events.extcall_memcpy_sem sz n gee cpvals m t Vundef m1)
+(BP: bind_parameters gee e m1 params vals m2) 
+j' tm3 j tm1 tm2 
+(MINJ : Mem.inject j' m2 tm3)
+(SEP : Events.inject_separated j j' m1 tm2),
+Events.inject_separated j j' m tm1.
+Proof. intros. inv MemCPY.
+  intros bb; intros.
+     unfold Events.inject_separated in SEP.
+     destruct (SEP _ _ _ H7 H8).
+     split; intros XX.  
+       apply H9. eapply Mem.storebytes_valid_block_1; eauto.
+     assert (~ Mem.valid_block m2 bb).
+       intros ZZ. apply H9.  apply (bind_parameters_validblock_2 _ _ _ _ _ _ BP _ ZZ). 
+       unfold Mem.inject in MINJ. destruct MINJ.
+         rewrite (mi_freeblocks _ H11) in H8. inv H8.    
+Qed.
+
+Lemma MS_store_parameters_correct:
+  forall e lenv te m1 params vl m2,
+  bind_parameters ge e m1 params vl m2 ->
+  forall s j1 cenv tf sp lo hi cs tm1 fn' k,
+  vars_vals_match j1 params vl te ->
+  list_norepet (List.map variable_name params) ->
+  Mem.inject j1 m1 tm1 ->
+  match_callstack prog j1 m1 tm1 (Frame cenv tf e lenv te sp lo hi :: cs) (Mem.nextblock m1) (Mem.nextblock tm1) ->
+  store_parameters cenv params = OK s ->
+ exists j2, exists tm2,
+     corestep_star CMin_core_sem tge (CMin_State fn' s k (Vptr sp Int.zero) te) tm1
+                 (CMin_State fn' Sskip k (Vptr sp Int.zero) te) tm2
+  /\ Mem.inject j2 m2 tm2
+  /\ match_callstack prog j2 m2 tm2 (Frame cenv tf e lenv te sp lo hi :: cs) (Mem.nextblock m2) (Mem.nextblock tm2)
+  /\ inject_incr j1 j2
+(********* The following 3 conditions are new*****)
+  /\ Events.inject_separated j1 j2 m1 tm1
+  /\ (forall b, Mem.valid_block m1 b -> Mem.valid_block m2 b)
+  /\ (forall b, Mem.valid_block tm1 b -> Mem.valid_block tm2 b).
+Proof.
+  induction 1.
+  (* base case *)
+  intros; simpl. monadInv H3. rename m into m1.
+  exists j1. exists tm1. split. eapply corestep_star_zero.
+       split; trivial.
+       split; trivial.
+       split; trivial.
+       split. apply inject_separated_same_meminj.
+       split; trivial.
+  (* scalar case *)
+  rename m1 into mm1. rename m into m1.
+  intros until k.  intros VVM NOREPET MINJ MATCH STOREP.
+  monadInv STOREP. inv VVM. inv NOREPET. 
+  exploit MS_var_set_self_correct_scalar; eauto.
+    econstructor; eauto. econstructor; eauto.
+  intros [tmm1 [EXEC1 [MINJ1 [MATCH1 [VB TVB]]]]]. 
+  exploit IHbind_parameters; eauto.
+  intros [j2 [tm2 [EXEC2 [MINJ2 [MATCH2 [INJ2 [SEP2 [VB2 TVB2]]]]]]]]. 
+  exists j2; exists tm2.
+  split. eapply corestep_star_trans; eauto.
+  split; trivial.
+  split; trivial.
+  split; trivial.
+  split.
+      intros bb; intros. destruct (SEP2 _ _ _ H3 H4).
+      split; intros N. (*rewrite VB in N. apply (H7 N).*) apply H7. apply (VB _ N).
+                                (*rewrite TVB in N. apply (H9 N). *) apply H9. apply (TVB _ N).
+  split; intros.   (*rewrite VB. apply VB2. *) apply VB2. apply (VB _ H3).
+           apply TVB2. (*rewrite <- TVB. assumption. *) apply (TVB _ H3).
+  (* array case *)
+  intros until k.  intros VVM NOREPET MINJ MATCH STOREP.
+  monadInv STOREP. inv VVM. inv NOREPET.
+  exploit MS_var_set_self_correct_array; eauto.
+  intros [f2 [tm2 [EXEC1 [MINJ1 [MATCH1 [INCR1 [UcOn [TUcOn1 [SEP1 [VB1 TVB1]]]]]]]]]].
+  clear UcOn TUcOn1. (*this shows that the first 2 new conditions of MS_var_set_self_correct_array are in fact superfluous*)
+  exploit IHbind_parameters. eapply vars_vals_match_incr; eauto. auto. eauto. eauto. eauto. 
+  intros [f3 [tm3 [EXEC2 [MINJ2 [MATCH2 [INCR2 [SEP2 [VB2 TVB2]]]]]]]]. 
+  exists f3; exists tm3.
+  split. eapply corestep_star_trans; eauto.
+  split. auto. split. auto. 
+  split. eapply inject_incr_trans; eauto.
+  split. clear EXEC2 MATCH2 EXEC1 MATCH1 IHbind_parameters.
+     intros bb; intros.
+       remember (f2 bb) as z; destruct z; apply eq_sym in Heqz.
+       (*Some p*) destruct p.
+             assert (f3 bb = Some (b0, z)). apply INCR2 in Heqz. assumption.
+             rewrite H6 in H3. inv H3.
+             eapply SEP1. assumption. eassumption.
+       (*None*) 
+             destruct (SEP2 _ _ _ Heqz H3).
+             split; intros N. (*rewrite VB1 in N. apply (H6 N).*) apply H6. apply (VB1 _ N).
+                 apply TVB1 in N. apply (H7 N).
+  split; intros. (*rewrite VB1. apply VB2.*) apply VB2. apply (VB1 _ H2).
+           apply TVB2. apply (TVB1 _ H2).
+Qed. 
+
+(***** All the additional conditions in the above auxiliary lemmas were needed for proving
+ the condition Events.inject_separated j j' m tmt in his lemma; otherwise, the claim is as before, 
+  just updated by replacing star step by corestep_star, as ususal*)
+Lemma MS_function_entry_ok:
+  forall tf fn m e m1 vargs m2 j cs tm cenv tm1 sp tvargs s fn' k,
+  list_norepet (fn_params_names fn ++ fn_vars_names fn) ->
+  alloc_variables empty_env m (fn_variables fn) e m1 ->
+  bind_parameters ge e m1 fn.(Csharpminor.fn_params) vargs m2 ->
+  match_callstack prog j m tm cs (Mem.nextblock m) (Mem.nextblock tm) ->
+  build_compilenv gce fn = (cenv, tf.(fn_stackspace)) ->
+  tf.(fn_stackspace) <= Int.max_unsigned ->
+  Mem.alloc tm 0 tf.(fn_stackspace) = (tm1, sp) ->
+  let tparams := List.map for_var (fn_params_names fn) in
+  let tvars := List.map for_var (fn_vars_names fn) in
+  let ttemps := List.map for_temp (Csharpminor.fn_temps fn) in
+  let te := set_locals (tvars ++ ttemps) (set_params tvargs tparams) in
+  val_list_inject j vargs tvargs ->
+  Mem.inject j m tm ->
+  store_parameters cenv fn.(Csharpminor.fn_params) = OK s ->
+  exists j', exists tm2,
+     corestep_star CMin_core_sem tge (CMin_State fn' s k (Vptr sp Int.zero) te) tm1
+                                 (CMin_State fn' Sskip k (Vptr sp Int.zero) te) tm2
+  /\ Mem.inject j' m2 tm2
+  /\ inject_incr j j'
+
+  (*This condition is new*)
+  /\ Events.inject_separated j j' m tm
+
+  /\ match_callstack prog j' m2 tm2
+       (Frame cenv tf e empty_temp_env te sp (Mem.nextblock m) (Mem.nextblock m1) :: cs)
+       (Mem.nextblock m2) (Mem.nextblock tm2).
+Proof.
+  intros.
+  exploit MS_match_callstack_alloc_variables; eauto.
+  intros [j1 [INCR1 [MINJ1 [MATCH1 [VB1 [SP1 SEP1]]]]]].
+  exploit vars_vals_match_holds.
+    eexact H. 
+    apply val_list_inject_incr with j. eauto. eauto.
+    eapply bind_parameters_normalized; eauto.
+  instantiate (1 := Csharpminor.fn_temps fn). 
+  fold tvars. fold ttemps. fold (fn_params_names fn). fold tparams. fold te.   
+  intro VVM.
+  exploit MS_store_parameters_correct.
+    eauto. eauto. eauto. eapply list_norepet_append_left; eauto.
+    eexact MINJ1. eexact MATCH1. eauto.
+  intros [j2 [tm2 [EXEC [MINJ2 [MATCH2 [INCR2 [SEP2 [VB2 TVB2]]]]]]]].
+  exists j2; exists tm2. 
+  split; eauto. split; auto. split; auto. eapply inject_incr_trans; eauto.
+Qed.
+
+Lemma MS_step_case_InternalCall:
+forall cenv  f j m tm e cs k tk vargs targs x m1 m2
+(Param: list_norepet (fn_params_names f ++ fn_vars_names f))
+(AllocVars : alloc_variables empty_env m (fn_variables f) e m1)
+(BindParams : bind_parameters ge e m1 (Csharpminor.fn_params f) vargs m2)
+(MINJ : Mem.inject j m tm)
+(MCS : match_callstack prog j m tm cs (Mem.nextblock m) (Mem.nextblock tm))
+(MK : match_cont k tk (fn_return f) cenv nil cs)
+(ISCC: Csharpminor.is_call_cont k)
+(ARGSINJ : val_list_inject j vargs targs)
+(EQ : transl_function gce f = OK x),
+exists c2' : CMin_core,
+  exists m2' : mem,
+       corestep_plus CMin_core_sem tge (CMin_Callstate (AST.Internal x) targs tk) tm c2' m2' /\
+  exists j' : meminj,
+        inject_incr j j' /\
+        (*again, have inject-sparatated here, as per definition of match relation*) 
+         Events.inject_separated j j' m tm /\
+  exists c',
+        inj_match_states_star unit match_cores MC_measure (tt,c') j'
+           (CSharpMin_State f (Csharpminor.fn_body f) k e empty_temp_env) m2 c2' m2'.
+Proof. intros.
+  generalize EQ; clear EQ; unfold transl_function.
+  caseEq (build_compilenv gce f). intros ce sz BC.
+  destruct (zlenv sz Int.max_unsigned); try congruence.
+  intro TRBODY.
+  generalize TRBODY; intro TMP. monadInv TMP.
+  set (tf := mkfunction (Csharpminor.fn_sig f) 
+                        (List.map for_var (fn_params_names f))
+                        (List.map for_var (fn_vars_names f)
+                         ++ List.map for_temp (Csharpminor.fn_temps f))
+                        sz
+                        (Sseq x1 x0)) in *.
+  caseEq (Mem.alloc tm 0 (fn_stackspace tf)). intros tm' sp ALLOC'.
+  exploit MS_function_entry_ok; eauto; simpl; auto.  
+  intros [j' [tm2 [EXEC [MINJ2 [IINCR [SEP2 MCS2]]]]]].
+  eexists; eexists; split.
+    eapply corestep_plus_star_trans.
+      eapply corestep_plus_one. eapply CompCertStep_CMin_corestep'. constructor; simpl; eauto. reflexivity.  
+    simpl.
+    eapply corestep_star_trans.
+      eapply corestep_star_one. eapply CompCertStep_CMin_corestep'. constructor. reflexivity.
+    simpl.
+    eapply corestep_star_trans. apply EXEC.
+      simpl. eapply corestep_star_one. eapply CompCertStep_CMin_corestep'. constructor. reflexivity.
+  simpl in *.
+  exists j'. split. assumption.
+  split. assumption.
+  exists (CSharpMin_State f(Csharpminor.fn_body f) k e empty_temp_env).
+  left.
+  econstructor. eexact TRBODY. eauto. eexact MINJ2. 
+  eexact MCS2.
+  inv MK; simpl in ISCC; contradiction || econstructor; eauto.
+Qed.
+
+(******************End of updated section for internal call rule*****************************)
+(************************************************************************************)
+
+Lemma MS_step_case_Return:
+forall j m tm cs f e lenv k tk ty cenv v tv optid
+(MINJ : Mem.inject j m tm)
+(MCS : match_callstack prog j m tm cs (Mem.nextblock m) (Mem.nextblock tm))
+(MK : match_cont (Csharpminor.Kcall optid f e lenv k) tk ty cenv nil cs)
+(RESINJ : val_inject j v tv),
+exists c2' : CMin_core,
+  exists m2' : mem,
+       corestep_plus CMin_core_sem tge (CMin_Returnstate tv tk) tm c2' m2'  /\
+    exists c', 
+       inj_match_states_star unit match_cores MC_measure (tt,c') j
+             (CSharpMin_State f Csharpminor.Sskip k e (set_optvar optid v lenv)) m c2' m2' .
+Proof. intros.
+  inv MK. simpl.
+  eexists; eexists; split.
+       eapply corestep_plus_one. eapply CompCertStep_CMin_corestep'. econstructor; eauto. reflexivity.
+  simpl.
+  exists  (CSharpMin_State f Csharpminor.Sskip k e (set_optvar optid v lenv)).
     left. unfold set_optvar. destruct optid; simpl option_map; econstructor; eauto.              
          eapply match_callstack_set_temp; eauto. 
 Qed. 
@@ -1811,7 +2870,7 @@ destruct H0.
          destruct c2; simpl in *; try inv H8.
          rename f0 into tfn. rename e0 into te. rename k0 into tk.
          exists  (CMin_State tfn x (Kseq x0 tk) (Vptr sp Int.zero) te). exists m2. 
-         exists (tt,CSharpMin_State f s (Csharpminor.Kseq s2 k) e le).
+         exists (tt,CSharpMin_State f s (Csharpminor.Kseq s2 k) e lenv).
          exists j. 
                 split. apply inject_incr_refl.
                 split. apply inject_separated_same_meminj.
@@ -1820,7 +2879,7 @@ destruct H0.
                           econstructor; eauto.
                      apply corestep_plus_one. eapply CompCertStep_CMin_corestep.  econstructor. reflexivity.
        (* seq 2 *)
-          exists c2. exists m2. exists (tt,CSharpMin_State f s (Csharpminor.Kseq s2 k) e le). exists j.
+          exists c2. exists m2. exists (tt,CSharpMin_State f s (Csharpminor.Kseq s2 k) e lenv). exists j.
                 split. apply inject_incr_refl.
                 split. apply inject_separated_same_meminj. 
                 destruct  c2; simpl in *; inv H9.
@@ -2071,7 +3130,7 @@ Qed.
      eapply MC_matchstates in MCS.
     assert (ZZ:= MC_matchstates _ _ _ _ _ _ _ MCS).
 (*   destruct c1; destruct c1'. simpl in H.*)
-   destruct (corestep_CompCertStep ge (CSharpMin_State f s k e le) m1 (CSharpMin_State f0 s0 k0 e0 le0) m1' H) as [t Ht]. simpl in *.
+   destruct (corestep_CompCertStep ge (CSharpMin_State f s k e lenv) m1 (CSharpMin_State f0 s0 k0 e0 le0) m1' H) as [t Ht]. simpl in *.
    assert (X:= transl_step_correct _ _ TRANSL _ _ _ Ht). simpl in X.
    inv H0; simpl in *. Focus 2.
    inv H. simpl in *.
