veric/Sim_starplus.v
@@ -18,17 +18,16 @@ Section Sim_EQ_SIMU_DIAGRAMS.
           {ge2:G2}
           {entry_points : list (val * val * signature)}.
 
-  Variable core_data:Type.
-  Variable order: core_data -> core_data -> Prop.
-  Hypothesis order_wf: well_founded order.
+  Let core_data := C1.
 
   Variable match_cores: core_data -> C1 -> C2 -> Prop.
+
   Hypothesis match_initial_cores: 
         forall v1 v2 sig, In (v1,v2,sig) entry_points ->
         forall vals,  Forall2 (Val.has_type) vals (sig_args sig) ->
-       exists cd : core_data, exists c1 : C1, exists c2 : C2,
+        exists c1 : C1, exists c2 : C2,
                 make_initial_core Sem1 ge1 v1 vals = Some c1 /\
-                make_initial_core Sem2 ge2 v2 vals = Some c2 /\ match_cores cd c1 c2.
+                make_initial_core Sem2 ge2 v2 vals = Some c2 /\ match_cores c1 c1 c2.
 (*Smallstep/old version of this file had
   Hypothesis match_initial_cores: 
         forall v1 v2 sig, In (v1,v2,sig) entry_points ->
@@ -46,289 +45,87 @@ But the core_initial axiom in the record Sim_eq.Forward_simulation_equals curren
       safely_halted Sem1 ge1 c1 = Some v -> safely_halted Sem2 ge2 c2 = Some v.
 
   Hypothesis eq_at_external: 
-         forall (d : core_data) (st1 : C1) (st2 : C2) (e : external_function) (args : list val) sig,
-         match_cores d st1 st2 ->
-         at_external Sem1 st1 = Some (e, sig, args) ->
-         at_external Sem2 st2 = Some (e, sig, args) /\
-         Forall2 Val.has_type args (sig_args sig).
+   forall (d : C1) (st1 : core_data) (st2 : C2) (e : external_function) (args : list val) (ef_sig : signature),
+    (d = st1 /\ match_cores d st1 st2) ->
+    at_external Sem1 st1 = Some (e, ef_sig, args) ->
+    (at_external Sem2 st2 = Some (e, ef_sig, args) /\
+     Forall2 Val.has_type args (sig_args ef_sig)).
 
-  Hypothesis eq_after_external: forall (d : core_data) (st1 : C1) (st2 : C2) (ret : val)
-                                                                 (e : external_function) (args : list val) sig,
-                      match_cores d st1 st2 ->
-                      at_external Sem1 st1 = Some (e, sig, args) ->
-(*                      at_external Sem2 st2 = Some (e, sig, args) ->
-                      Forall2 Val.has_type args (sig_args (ef_sig e)) ->*)
-                      Val.has_type ret (proj_sig_res sig) ->
-(*                      Val.has_type ret (proj_sig_res (ef_sig e)) ->*)
-(*
-                      at_external Sem1 st1 = Some (e, sig, args) ->
-                      at_external Sem2 st2 = Some (e, sig, args) ->
-                      Forall2 Val.has_type args (sig_args sig) ->
-                      Val.has_type ret (proj_sig_res sig) ->
-*)
-                      exists st1' : C1, exists st2' : C2, exists d' : core_data,
-                              after_external Sem1 (Some ret) st1 = Some st1' /\
-                              after_external Sem2 (Some ret) st2 = Some st2' /\ match_cores d' st1' st2'.
-(*
-Section SIMULATION_STAR_WF.
+Hypothesis eq_after_external:
+   forall (d : C1) (st1 : core_data) (st2 : C2) (ret : val) (e : external_function) (args : list val) (ef_sig : signature),
+    (d = st1 /\ match_cores d st1 st2) ->
+    at_external Sem1 st1 = Some (e, ef_sig, args) ->
+    at_external Sem2 st2 = Some (e, ef_sig, args) ->
+    Forall2 Val.has_type args (sig_args ef_sig) ->
+    Val.has_type ret (proj_sig_res ef_sig) ->
+    exists st1', exists st2', exists d',
+      after_external Sem1 (Some ret) st1 = Some st1' /\
+      after_external Sem2 (Some ret) st2 = Some st2' /\
+      d' = st1' /\ match_cores d' st1' st2'.
+
+Section EQ_SIMULATION_STAR_WF.
+Variable order: C1 -> C1 -> Prop.
+Hypothesis order_wf: well_founded order.
+
   Hypothesis eq_simulation:
      forall c1 m c1' m',  corestep Sem1 ge1 c1 m c1' m' ->
-     forall d c2, match_cores d c1 c2 ->
-      exists c2', exists d', match_cores d' c1' c2' /\
-                  (corestep_plus Sem2 ge2  c2 m c2' m' \/ (corestep_star Sem2 ge2 c2 m c2' m' /\ order d' d)).
+     forall c2, match_cores c1 c1 c2 ->
+      exists c2', match_cores c1' c1' c2' /\
+                  (corestep_plus Sem2 ge2  c2 m c2' m' \/ (corestep_star Sem2 ge2 c2 m c2' m' /\ order c1' c1)).
 
 Lemma  eq_simulation_star_wf: Sim_eq.Forward_simulation_equals _ _ Sem1 Sem2 ge1 ge2 entry_points.
 Proof.
   eapply Sim_eq.Build_Forward_simulation_equals with
         (core_ord := order)
-        (match_core := match_cores). (*fun d c1 c2 => idx = s1 /\ match_cores c1 c2);*)
+        (match_core := fun d c1 c2 => d = c1 /\ match_cores d c1 c2).
    apply order_wf.
-   apply eq_simulation.
-   apply match_initial_cores.
-   apply eq_safely_halted.
+   intros. destruct H0; subst.  destruct (eq_simulation _ _ _ _ H _ H1) as [c2' [MC' Step]].
+                  exists c2'.  exists st1'.  split; eauto. clear eq_simulation eq_after_external eq_at_external .
+   intros. destruct (match_initial_cores _ _ _ H _ H0) as [c1' [c2' [MIC1 [MIC2 MC]]]].
+                 exists c1'. exists c1'. exists c2'. split; eauto.
+   intros.  clear eq_simulation eq_after_external eq_at_external . destruct H; subst.
+                eapply eq_safely_halted; eauto.
    apply eq_at_external.
    apply eq_after_external.
 Qed.
-End SIMULATION_STAR_WF.
+End EQ_SIMULATION_STAR_WF.
 
-Section SIMULATION_STAR.
+Section EQ_SIMULATION_STAR.
   Variable measure: C1 -> nat.
   
   Hypothesis eq_star_simulation:
     forall c1 m c1' m', corestep Sem1 ge1 c1 m c1' m'  -> 
-    (measure c1' < measure c1 /\
-    forall d c2, match_cores d c1 c2 ->
-    (exists c2', exists d', corestep_plus Sem2 ge2 c2 m c2' m' /\ match_cores d' c1' c2' /\ order d' d)
-   \/ (measure c1' < measure c1 /\ m'=m /\ match_cores d c1' c2))%nat.
-
-  Definition star_data : Type := (core_data * C1)%type.
-  Definition star_ord:= lex_ord order (ltof _ measure). 
-
-  Definition match_cores_star (cd:star_data) (c1:  C1) (c2: C2): Prop :=
-       match cd with (d,c) => match_cores d c1 c2 \/exists d',  order d' d /\ match_cores d' c c2 (* lt (measure c1) (measure c) /\*)
-       end.
-(*
-  Definition match_cores_star (cd:star_data) (c1:  C1) (c2: C2): Prop :=
-       match cd with (d,c) => match_cores d c1 c2 /\ lt (measure c1) (measure c) 
-       end.
-*)
-Lemma  eq_simulation_star: Sim_eq.Forward_simulation_equals _ _ Sem1 Sem2 ge1 ge2 entry_points.
-Proof.
-  eapply Sim_eq.Build_Forward_simulation_equals with (core_ord:= star_ord)(match_core:=match_cores_star).
-      eapply wf_lex_ord. apply order_wf. apply (well_founded_ltof _ measure).
-      clear match_initial_cores eq_safely_halted eq_at_external eq_after_external.
-         unfold match_cores_star. intros. destruct d as [d c].
-         rename st1 into c1. rename st1' into c1'. rename st2 into c2.
-        destruct  (eq_star_simulation _ _ _ _ H) as [MM LLL]; clear eq_star_simulation .
-        destruct H0.
-        (*1*) specialize (LLL _ _ H0).
-                              destruct LLL as [X | X]. (*; clear LLL. eq_star_simulation.*)
-                                  (*case 1*) destruct X as [c2' [d'' [CS [MC ORD]]]].
-                                                    exists c2'. exists (d'', c). split. left. assumption.  left; assumption. (*transitivity*)  (*left; trivial. left; trivial.*)                                                   
-                                 (*case 2*) destruct X as [Measure [M MTCH]]. subst.
-                                                    exists c2.  unfold star_ord.  exists (d, c1). split. left; trivial. 
-                                                                      (*exists d.  split; trivial. left; assumption.*) (*left; assumption. *)(* right; auto*)
-                                                             right. split. exists O. reflexivity.
-                                                                 apply lex_ord_right. apply H1.  (*unfold ltof. admit.*)  (*HERE's A HOLE!!*)
-            (*destruct H0. admit.*)
-    clear eq_star_simulation eq_after_external eq_at_external eq_safely_halted.
-        intros. specialize (match_initial_cores _ _ _ H _ H0).
-                   destruct match_initial_cores as [d [c1 [c2 [Ini1 [Ini2 MC]]]]].
-                   exists (d,c1). exists c1. exists c2. split; trivial. split; trivial.
-                   simpl. left; trivial.
-    clear eq_star_simulation eq_after_external eq_at_external match_initial_cores.
-        intros. destruct cd as [d c].
-                   destruct H. eapply (eq_safely_halted _ _ _ _ H H0).
-                   destruct H.  admit. (*HOLE*)
-    clear eq_after_external match_initial_cores eq_star_simulation eq_safely_halted.
-        intros. destruct d as [d c].
-                   destruct H. 
-                       eapply eq_at_external. apply H. apply H0.
-                   destruct H.  
-                       eapply eq_at_external. apply H1. admit. (*HOLE*)
-       (*afterexternal*)
-           admit.
-Qed.
-End SIMULATION_STAR.
-*)
-
-Section EQ_SIMULATION_STAR.
-  Variable measure: C1 -> nat. 
-  Definition star_data : Type := (core_data * C1)%type.
-  Definition star_ord:= lex_ord order (ltof _ measure).
- 
-  Definition match_cores_star (cd:star_data) (c1:  C1) (c2: C2): Prop :=
-       match cd with (d,c) => match_cores d c1 c2 \/ (lt (measure c) (measure c1) /\ match_cores d c c2)
-       end.
-
-  Hypothesis eq_star_halted_Zero:  forall c1 v, safely_halted Sem1 ge1 c1 = Some v -> measure c1 = O.
-  Hypothesis eq_star_atExt_Zero:  forall c1 v, at_external Sem1 c1 = Some v -> measure c1 = O.
-
-(*  Hypothesis eq_star_simulation:
-     forall c1 m c1' m',  corestep Sem1 ge1 c1 m c1' m' ->
-     forall d c2, match_cores d c1 c2 ->
-      exists c2', exists d', (corestep_plus Sem2 ge2 c2 m c2' m' /\ match_cores_star (d',c1') c1' c2' /\ order d' d) \/
-                                       (corestep_star Sem2 ge2 c2 m c2' m' /\ measure c1' < measure c1 /\ m'=m /\ match_cores d c1' c2)%nat.
-*)(*
-  Hypothesis  eq_star_simulation: forall c1 m c1' m' (CS: corestep Sem1 ge1 c1 m c1' m')
-                       dc c2 (MCS:match_cores_star dc c1 c2),
-                      exists c2', 
-                            (exists dc', match_cores_star dc' c1' c2' /\ corestep_plus Sem2 ge2 c2 m c2' m') \/
-                            (exists d, exists c, dc=(d,c) /\ measure c1 < measure c1' /\ 
-                                     match_cores_star (d,c) c1' c2)%nat.*)
- Hypothesis eq_star_sim_diag:  forall c1 m c1' m' (CS: corestep Sem1 ge1 c1 m c1' m')
-                       dc c2 (MCS:match_cores_star dc c1 c2),
-                      exists c2', exists dc',
-    match_cores_star dc' c1' c2' /\
-    (corestep_plus Sem2 ge2 c2 m c2' m' \/
-     corestep_star Sem2 ge2 c2 m c2' m' /\ star_ord dc' dc).
+    forall c2, match_cores c1 c1 c2 ->
+      (exists c2', corestep_plus Sem2 ge2 c2 m c2' m' /\ match_cores c1' c1' c2')
+     \/ (measure c1' < measure c1 /\ m=m' /\ match_cores c1' c1' c2)%nat.
 
 Lemma  eq_simulation_star: Sim_eq.Forward_simulation_equals _ _ Sem1 Sem2 ge1 ge2 entry_points.
 Proof.
-  eapply Sim_eq.Build_Forward_simulation_equals with (core_ord:= star_ord)(match_core:=match_cores_star).
-      eapply wf_lex_ord. apply order_wf.  apply (well_founded_ltof _ measure).
-   apply eq_star_sim_diag.
-   intros. clear  eq_safely_halted eq_at_external eq_after_external eq_star_sim_diag.
-          specialize (match_initial_cores _ _ _ H _ H0).
-          destruct match_initial_cores as [d [c1 [c2 [Ini1 [Ini2 Mtch]]]]]; clear match_initial_cores.
-          exists (d,c1). exists c1. exists c2. split; trivial.  split; trivial.  left.  trivial.
-   intros. clear  eq_at_external eq_after_external eq_star_sim_diag match_initial_cores eq_star_sim_diag.
-        assert (X:= eq_star_halted_Zero _ _ H0).
-         destruct cd as [d c]. destruct H. eapply eq_safely_halted . apply H. apply H0.
-         destruct H. rewrite X in H. inv H.
-   intros. clear eq_star_sim_diag eq_safely_halted  eq_after_external match_initial_cores eq_star_halted_Zero.
-           assert (X:= eq_star_atExt_Zero _ _ H0).
-        destruct d as [d c]. destruct H.
-          eapply eq_at_external ; eauto. 
-        destruct H. rewrite X in H. inv H.
-   intros. clear eq_star_sim_diag eq_safely_halted  match_initial_cores eq_star_halted_Zero.
-           destruct d as [d c]. 
-           destruct H. specialize (eq_after_external _ _ _ _ _ _ _ H H0 H3).
-              (* specialize (eq_after_external _ _ _ _ _ _ H H0 H1 H2 H3).*)
-(*
-           destruct H. specialize (eq_after_external _ _ _ _ _ _ _ H H0 H1 H2 H3).
-*)
-                destruct eq_after_external  as [c1' [c2' [d' [AftExt1 [AftExt2 MC]]]]].
-                exists c1'. exists c2'. exists (d',c). split; trivial. split; trivial. left. assumption.
-          destruct H. rewrite (eq_star_atExt_Zero _ _ H0) in H. inv H.
+  eapply eq_simulation_star_wf. apply  (well_founded_ltof _ measure).
+        intros. destruct (eq_star_simulation _ _ _ _ H _ H0).
+             destruct H1 as [c2' [CSP MC']]. exists c2'. split; trivial. left; trivial.
+             destruct H1 as [X1 [X2 X3]]; subst. exists c2. split; trivial. right. split; trivial.
+             eapply corestep_star_zero. 
 Qed.
 End EQ_SIMULATION_STAR.
 
-(** Simulation when one transition in the first program corresponds
-    to one or several transitions in the second program. *)
-
 Section EQ_SIMULATION_PLUS.
-(*
-Hypothesis simulation:
-  forall s1 t s1', Step L1 s1 t s1' ->
-  forall s2, match_states s1 s2 ->
-  exists s2', Plus L2 s2 t s2' /\ match_states s1' s2'.
-*)
- Hypothesis eq_plus_sim_diag:  forall c1 m c1' m' (CS: corestep Sem1 ge1 c1 m c1' m')
-                       dc c2 (MCS:match_cores_star (fun _ => O) dc c1 c2),
-                      exists c2', exists dc',
-    match_cores_star (fun _ => O) dc' c1' c2' /\ corestep_plus Sem2 ge2 c2 m c2' m'.
+  Variable measure: C1 -> nat. 
+  Hypothesis eq_plus_simulation:
+    forall c1 m c1' m', corestep Sem1 ge1 c1 m c1' m'  -> 
+    forall c2, match_cores c1 c1 c2 ->
+            exists c2', corestep_plus Sem2 ge2 c2 m c2' m' /\ match_cores c1' c1' c2'.
 
 Lemma  eq_simulation_plus: Sim_eq.Forward_simulation_equals _ _ Sem1 Sem2 ge1 ge2 entry_points.
 Proof.
-  apply eq_simulation_star with (measure := fun _ => O).
-      intros. trivial.
-      intros. trivial.
-      intros.
-               clear eq_after_external eq_at_external eq_safely_halted match_initial_cores.
-               destruct (eq_plus_sim_diag _ _ _ _ CS _ _ MCS) as [c2' [dc' [MCS' CSP]]].
-               exists c2'. exists dc'. split. assumption. left. trivial.
+  apply eq_simulation_star with (measure:=measure).
+        intros. destruct (eq_plus_simulation _ _ _ _ H _ H0).
+             left. eexists; eauto.
 Qed.
-
 End EQ_SIMULATION_PLUS.
-
-(*
- eq_safely_halted; eassumption.
-        destruct H. 
-   apply eq_safely_halted.
-   apply eq_at_external.
-   apply eq_after_external.
-   intros. clear match_initial_cores  eq_safely_halted eq_at_external eq_after_external.
-        destruct d as [d c]. inv H0. 
-        specialize (eq_star_simulation _ _ _ _ H _ _ H1). 
-         destruct eq_star_simulation  as [c2' [d' [ [StepPlus [MtchStar Ord]]| [StepStar [MM [X Mtch]]]]]]; clear eq_star_simulation.
-              exists c2'. exists (d',st1'). split; trivial. left; assumption.
-          subst. exists c2'. exists (d,
-
-   intros. clear match_initial_cores  eq_safely_halted eq_at_external eq_after_external.
-        specialize (eq_star_simulation _ _ _ _ H _ _ H0). 
-        destruct d as [d c]. inv H0.
-         destruct  eq_star_simulation as [c2' [X | X]]; clear eq_star_simulation.
-             destruct X as [[d' c'] [ MtchStar SPlus]].
-             exists c2'. exists (d',c'); split; trivial. left; trivial.
-           destruct X as [d' [c' [X [StepStar [MM Mtch]]]]]. inv X.
-              exists c2'.  exists (d',c'). split; trivial. left; assumption.
-          subst. exists c2'. exists (d,
-   apply eq_star_simulation.
-   intros. clear eq_star_simulation  eq_safely_halted eq_at_external eq_after_external.
-   intros. clear eq_star_simulation  eq_at_external eq_after_external match_initial_cores.
-        destruct cd as [d c]. destruct H.
-           eapply eq_safely_halted; eassumption.
-        destruct H. 
-   apply eq_safely_halted.
-   apply eq_at_external.
-   apply eq_after_external.
-   intros. clear match_initial_cores  eq_safely_halted eq_at_external eq_after_external.
-        destruct d as [d c]. inv H0. 
-        specialize (eq_star_simulation _ _ _ _ H _ _ H1). 
-         destruct eq_star_simulation  as [c2' [d' [ [StepPlus [MtchStar Ord]]| [StepStar [MM [X Mtch]]]]]]; clear eq_star_simulation.
-              exists c2'. exists (d',st1'). split; trivial. left; assumption.
-          subst. exists c2'. exists (d,
-  
-   apply eq_simulation.
-   apply match_initial_cores.
-   apply eq_safely_halted.
-   apply eq_at_external.
-   apply eq_after_external.
-Qed.
- 
-  Hypothesis eq_simulation:
-     forall c1 m c1' m',  corestep Sem1 ge1 c1 m c1' m' ->
-     forall d c2, match_cores d c1 c2 ->
-      exists c2', exists d', match_cores d' c1' c2' /\
-                  (corestep_plus Sem2 ge2  c2 m c2' m' \/ (corestep_star Sem2 ge2 c2 m c2' m' /\ order d' d)).
-
-Lemma  eq_simulation_star_wf: Sim_eq.Forward_simulation_equals _ _ Sem1 Sem2 ge1 ge2 entry_points.
-Proof.
-  eapply Sim_eq.Build_Forward_simulation_equals with
-        (core_ord := order)
-        (match_core := match_cores). (*fun d c1 c2 => idx = s1 /\ match_cores c1 c2);*)
-   apply order_wf.
-   apply eq_simulation.
-   apply match_initial_cores.
-   apply eq_safely_halted.
-   apply eq_at_external.
-   apply eq_after_external.
-Qed.
-End SIMULATION_STAR_WF.
-(** Simulation when one transition in the first program corresponds
-    to one or several transitions in the second program. *)
-Section SIMULATION_PLUS.
-
-Hypothesis eq_plus_simulation:
-  forall c1 m c1' m', corestep Sem1 ge1 c1 m c1' m'  ->
-  forall d c2, match_cores d c1 c2 ->
-  (exists c2', exists d', corestep_plus Sem2 ge2 c2 m c2' m' /\ match_cores d' c1' c2'  /\ order d' d).
-
-Lemma eq_simulation_plus: Sim_eq.Forward_simulation_equals _ _ Sem1 Sem2 ge1 ge2 entry_points.
-Proof.
-  apply eq_simulation_star with (measure := fun _ => O).
-  intros. left. clear eq_after_external eq_at_external  eq_safely_halted match_initial_cores.
-       apply (eq_plus_simulation _ _ _ _ H _ _ H0).
-Qed.
-
-End SIMULATION_PLUS.
-*)
-
 End Sim_EQ_SIMU_DIAGRAMS.
 
 Section Sim_EXT_SIMU_DIAGRAMS.
-
   Context {G1 C1 D1 G2 C2 D2:Type}
           {Sem1 : CompcertCoreSem G1 C1 D1}
           {Sem2 : CompcertCoreSem G2 C2 D2}
@@ -337,44 +134,43 @@ Section Sim_EXT_SIMU_DIAGRAMS.
           {ge2:G2}
           {entry_points : list (val * val * signature)}.
 
-  Variable core_data:Type.
-  Variable order: core_data -> core_data -> Prop.
-  Hypothesis order_wf: well_founded order.
+  Let core_data := C1.
 
-  Variable match_state: core_data -> C1 -> mem -> C2 -> mem -> Prop.
+  Variable match_states: core_data -> C1 -> mem -> C2 -> mem -> Prop.
+
   Hypothesis match_initial_cores: forall v1 v2 sig,
       In (v1,v2,sig) entry_points ->
         forall vals vals' m1 m2,
           Forall2 Val.lessdef vals vals' ->
           Forall2 (Val.has_type) vals' (sig_args sig) ->
           Mem.extends m1 m2 ->
-          exists cd, exists c1, exists c2,
+          exists c1, exists c2,
             make_initial_core Sem1 ge1 v1 vals = Some c1 /\
             make_initial_core Sem2 ge2 v2 vals' = Some c2 /\
-            match_state cd c1 m1 c2 m2.
+            match_states c1 c1 m1 c2 m2.
 
-  Hypothesis ext_safely_halted:
+Hypothesis ext_safely_halted:
       forall cd st1 m1 st2 m2 (v:int),
-        match_state cd st1 m1 st2 m2 ->
+        match_states cd st1 m1 st2 m2 ->
         safely_halted Sem1 ge1 st1 = Some v ->
           safely_halted Sem2 ge2 st2 = Some v /\
           Mem.extends m1 m2.
 
   Hypothesis ext_at_external: 
-      forall cd st1 m1 st2 m2 e vals1 sig,
-        match_state cd st1 m1 st2 m2 ->
-        at_external Sem1 st1 = Some (e,vals1) ->
-        exists vals2,
+        forall d st1 m1 st2 m2 e vals1 sig,
+          (d = st1 /\ match_states d st1 m1 st2 m2) ->
+         at_external Sem1 st1 = Some (e, sig, vals1) ->
+         exists vals2,
           Mem.extends m1 m2 /\
           Forall2 Val.lessdef vals1 vals2 /\
           Forall2 (Val.has_type) vals2 (sig_args sig) /\
-          at_external Sem2 st2 = Some (e,vals2).
+          at_external Sem2 st2 = Some (e,sig,vals2).
 
   Hypothesis ext_after_external:
-      forall cd st1 st2 m1 m2 e vals1 vals2 ret1 ret2 m1' m2' sig,
-        match_state cd st1 m1 st2 m2 ->
-        at_external Sem1 st1 = Some (e,vals1) ->
-        at_external Sem2 st2 = Some (e,vals2) ->
+      forall d st1 st2 m1 m2 e vals1 vals2 ret1 ret2 m1' m2' sig,
+        (d=st1 /\ match_states d st1 m1 st2 m2) ->
+        at_external Sem1 st1 = Some (e,sig,vals1) ->
+        at_external Sem2 st2 = Some (e,sig,vals2) ->
 
         Forall2 Val.lessdef vals1 vals2 ->
         Forall2 (Val.has_type) vals2 (sig_args sig) ->
@@ -387,95 +183,89 @@ Section Sim_EXT_SIMU_DIAGRAMS.
 
         Val.has_type ret2 (proj_sig_res sig) ->
 
-        exists st1', exists st2', exists cd',
+        exists st1', exists st2', exists d',
           after_external Sem1 (Some ret1) st1 = Some st1' /\
           after_external Sem2 (Some ret2) st2 = Some st2' /\
-          match_state cd' st1' m1' st2' m2'. 
+          d' = st1' /\ match_states d' st1' m1' st2' m2'. 
+
+Section EXT_SIMULATION_STAR_WF.
+Variable order: C1 -> C1 -> Prop.
+Hypothesis order_wf: well_founded order.
+
+  Hypothesis ext_simulation:
+     forall c1 m1 c1' m1',  corestep Sem1 ge1 c1 m1 c1' m1' ->
+     forall c2 m2, match_states c1 c1 m1 c2 m2 ->
+      exists c2', exists m2', match_states c1' c1' m1' c2' m2' /\
+                  (corestep_plus Sem2 ge2  c2 m2 c2' m2' \/ (corestep_star Sem2 ge2 c2 m2 c2' m2' /\ order c1' c1)).
+
+Lemma  ext_simulation_star_wf: Sim_ext.Forward_simulation_extends _ _ Sem1 Sem2 ge1 ge2 entry_points.
+Proof.
+  eapply Sim_ext.Build_Forward_simulation_extends with
+        (core_ord := order)
+        (match_state := fun d c1 m1 c2 m2 => d = c1 /\ match_states d c1 m1 c2 m2).
+   apply order_wf.
+   intros. destruct H0; subst.
+              destruct (ext_simulation _ _ _ _ H _ _ H1) as [c2' [m2' [MC' Step]]].
+              exists c2'. exists m2'. exists st1'.  split; eauto.
+   intros. destruct (match_initial_cores _ _ _ H _ _ _ _ H0 H1 H2) as [c1' [c2' [MIC1 [MIC2 MC]]]].
+                 exists c1'. exists c1'. exists c2'. split; eauto.
+   intros. destruct H; subst. eapply ext_safely_halted; eauto.
+   intros.  destruct H. eapply ext_at_external; eauto.
+   intros. destruct H. eapply ext_after_external; eauto.
+Qed.
+End EXT_SIMULATION_STAR_WF.
 
 Section EXT_SIMULATION_STAR.
-  Variable measure: C1 -> nat. 
-  Definition ext_star_data : Type := (core_data * C1)%type.
-  Definition ext_star_ord:= lex_ord order (ltof _ measure).
- 
-  Definition ext_match_states_star (cd:ext_star_data) (c1:  C1) m1 (c2: C2) m2 : Prop :=
-       match cd with (d,c) => match_state d c1 m1 c2 m2 \/ (lt (measure c) (measure c1) /\ match_state d c m1 c2 m2)
-       end.
-
-  Hypothesis ext_star_halted_Zero:  forall c1 v, safely_halted Sem1 ge1 c1 = Some v -> measure c1 = O.
-  Hypothesis ext_star_atExt_Zero:  forall c1 v, at_external Sem1 c1 = Some v -> measure c1 = O.
-
- Hypothesis ext_star_sim_diag:  forall c1 m1 c1' m1' (CS: corestep Sem1 ge1 c1 m1 c1' m1')
-                       dc c2 m2 (MCS:ext_match_states_star dc c1 m1 c2 m2),
-                      exists c2', exists m2', exists dc',
-    ext_match_states_star dc' c1' m1' c2' m2' /\
-    (corestep_plus Sem2 ge2 c2 m2 c2' m2' \/
-     corestep_star Sem2 ge2 c2 m2 c2' m2' /\ ext_star_ord dc' dc).
+  Variable measure: C1 -> nat.
+  
+  Hypothesis ext_star_simulation:
+    forall c1 m1 c1' m1', corestep Sem1 ge1 c1 m1 c1' m1'  -> 
+    forall c2 m2, match_states c1 c1 m1 c2 m2 ->
+      (exists c2', exists m2', corestep_plus Sem2 ge2 c2 m2 c2' m2' /\ match_states c1' c1' m1' c2' m2')
+     \/ (measure c1' < measure c1 /\ (*apparently not needed: Mem.extends m1' m2 /\ *) match_states c1' c1' m1' c2 m2)%nat.
 
 Lemma  ext_simulation_star: Sim_ext.Forward_simulation_extends _ _ Sem1 Sem2 ge1 ge2 entry_points.
 Proof.
-  eapply Sim_ext.Build_Forward_simulation_extends with (core_ord:= ext_star_ord). (*(match_state:=ext_match_states_star).*)
-      eapply wf_lex_ord. apply order_wf.  apply (well_founded_ltof _ measure).
-   apply ext_star_sim_diag.
-   intros. clear  ext_safely_halted ext_at_external ext_after_external ext_star_sim_diag.
-          specialize (match_initial_cores _ _ _ H _ _ _ _ H0 H1 H2).
-          destruct match_initial_cores as [d [c1 [c2 [Ini1 [Ini2 Mtch]]]]]; clear match_initial_cores.
-          exists (d,c1). exists c1. exists c2. split; trivial.  split; trivial.  left.  trivial.
-   intros. clear  ext_at_external ext_after_external ext_star_sim_diag match_initial_cores ext_star_sim_diag.
-        assert (X:= ext_star_halted_Zero _ _ H0).
-         destruct cd as [d c]. destruct H. eapply ext_safely_halted . apply H. apply H0.
-         destruct H. rewrite X in H. inv H.
-   intros. clear ext_star_sim_diag ext_safely_halted  ext_after_external match_initial_cores ext_star_halted_Zero.
-           assert (X:= ext_star_atExt_Zero _ _ H0).
-        destruct cd as [d c]. destruct H.
-          eapply ext_at_external ; eauto. 
-        destruct H. rewrite X in H. inv H.
-   intros. clear ext_star_sim_diag ext_safely_halted  match_initial_cores ext_star_halted_Zero ext_at_external.
-           destruct cd as [d c]. 
-           destruct H. specialize (ext_after_external _ _ _ _ _ _ _ _ _ _ _ _ _ H H0 H1 H2 H3 H4 H5 H6 H7 H8 H9).
-                destruct ext_after_external  as [c1' [c2' [d' [AftExt1 [AftExt2 MC]]]]].
-                exists c1'. exists c2'. exists (d',c). split; trivial. split; trivial. left. assumption.
-          destruct H. rewrite (ext_star_atExt_Zero _ _ H0) in H. inv H.
+  eapply ext_simulation_star_wf.
+        apply  (well_founded_ltof _ measure).
+        intros. destruct (ext_star_simulation _ _ _ _ H _ _ H0).
+             destruct H1 as [c2' [m2' [CSP MC']]]. exists c2'. exists m2'. split; trivial. left; trivial.
+             destruct H1 as [X1 X3]; subst. exists c2. exists m2. split; trivial. right. split; trivial.
+             eapply corestep_star_zero. 
 Qed.
 End EXT_SIMULATION_STAR.
 
 Section EXT_SIMULATION_PLUS.
- Hypothesis ext_plus_sim_diag:  forall c1 m1 c1' m1' (CS: corestep Sem1 ge1 c1 m1 c1' m1')
-                       dc c2 m2 (MCS:ext_match_states_star (fun _ => O) dc c1 m1 c2 m2),
-                      exists c2', exists m2', exists dc',
-    ext_match_states_star (fun _ => O) dc' c1' m1' c2' m2' /\ corestep_plus Sem2 ge2 c2 m2 c2' m2'.
+  Variable measure: C1 -> nat. 
+  Hypothesis ext_plus_simulation:
+    forall c1 m1 c1' m1', corestep Sem1 ge1 c1 m1 c1' m1'  -> 
+    forall c2 m2, match_states c1 c1 m1 c2 m2 ->
+            exists c2', exists m2', corestep_plus Sem2 ge2 c2 m2 c2' m2' /\ match_states c1' c1' m1' c2' m2'.
 
 Lemma  ext_simulation_plus: Sim_ext.Forward_simulation_extends _ _ Sem1 Sem2 ge1 ge2 entry_points.
 Proof.
-  apply ext_simulation_star with (measure := fun _ => O).
-      intros. trivial.
-      intros. trivial.
-      intros.
-               clear ext_after_external ext_at_external ext_safely_halted match_initial_cores.
-               destruct (ext_plus_sim_diag _ _ _ _ CS _ _ _ MCS) as [c2' [m2' [dc' [MCS' CSP]]]].
-               exists c2'. exists m2'. exists dc'. split. assumption. left. trivial.
+  apply ext_simulation_star with (measure:=measure).
+        intros. destruct (ext_plus_simulation _ _ _ _ H _ _ H0).
+             left. eexists; eauto.
 Qed.
-
 End EXT_SIMULATION_PLUS.
-
 End Sim_EXT_SIMU_DIAGRAMS.
 
 Section Sim_INJ_SIMU_DIAGRAMS.
-
   Context {F1 V1 C1 D1 G2 C2 D2:Type}
           {Sem1 : CompcertCoreSem (Genv.t F1 V1)  C1 D1}
           {Sem2 : CompcertCoreSem G2 C2 D2}
 
           {ge1: Genv.t F1 V1} 
           {ge2:G2}
-          {entry_points : list (val * val * signature)}.
+          {entry_points : list (val * val * signature)}. 
 
-  Variable core_data:Type.
-  Variable order: core_data -> core_data -> Prop.
-  Hypothesis order_wf: well_founded order.
+  Let core_data := C1.
 
-  Variable match_state: core_data -> meminj ->  C1 -> mem -> C2 -> mem -> Prop.
+  Variable match_states: core_data -> meminj -> C1 -> mem -> C2 -> mem -> Prop.
+
   Hypothesis match_initial_cores: forall v1 v2 sig,
-       In (v1,v2,sig) entry_points -> 
+        In (v1,v2,sig) entry_points -> 
        forall vals1 c1 m1 j vals2 m2,
           make_initial_core Sem1 ge1 v1 vals1 = Some c1 ->
           Mem.inject j m1 m2 -> 
@@ -483,33 +273,34 @@ Section Sim_INJ_SIMU_DIAGRAMS.
            Forall2 (val_inject j) vals1 vals2 ->
 
           Forall2 (Val.has_type) vals2 (sig_args sig) ->
-          exists cd, exists c2, (*exists vals2, exists m2, *)
+          exists c2, (*exists vals2, exists m2, *)
             make_initial_core Sem2 ge2 v2 vals2 = Some c2 /\
-            match_state cd j c1 m1 c2 m2. 
+            match_states c1 j c1 m1 c2 m2. 
 
   Hypothesis inj_safely_halted:forall cd j c1 m1 c2 m2 (v1:int),
-      match_state cd j c1 m1 c2 m2 ->
+      match_states cd j c1 m1 c2 m2 ->
       safely_halted Sem1 ge1 c1 = Some v1 ->
         (safely_halted Sem2 ge2 c2 = Some v1 /\
          Mem.inject j m1 m2).
 
   Hypothesis inj_at_external: 
-      forall cd j st1 m1 st2 m2 e vals1 sig,
-        match_state cd j st1 m1 st2 m2 ->
-        at_external Sem1 st1 = Some (e,vals1) ->
+      forall d j st1 m1 st2 m2 e vals1 sig,
+        d = st1 /\ match_states d j st1 m1 st2 m2 ->
+        at_external Sem1 st1 = Some (e,sig,vals1) ->
         ( Mem.inject j m1 m2 /\
           meminj_preserves_globals ge1 j /\ (*LENB: also added meminj_preserves_global HERE*)
           exists vals2, Forall2 (val_inject j) vals1 vals2 /\
           Forall2 (Val.has_type) vals2 (sig_args sig) /\
-          at_external Sem2 st2 = Some (e,vals2)).
+          at_external Sem2 st2 = Some (e,sig,vals2)).
 
   Hypothesis inj_after_external:
-      forall cd j j' st1 st2 m1 e vals1 (*vals2*) ret1 m1' m2 m2' ret2 sig,
-        Mem.inject j m1 m2->
-        match_state cd j st1 m1 st2 m2 ->
-        at_external Sem1 st1 = Some (e,vals1) ->
-(*     at_external Sem2 st2 = Some (e,vals2) ->
-        Forall2 (val_inject j) vals1 vals2 ->*)
+      forall d j j' st1 st2 m1 e vals1 (*vals2*) ret1 m1' m2 m2' ret2 sig,
+        (d=st1 /\ match_states d j st1 m1 st2 m2) ->
+        at_external Sem1 st1 = Some (e,sig,vals1) ->
+(*     at_external Sem2 st2 = Some (e,sig,vals2) ->
+        Forall2 (Val.has_type) vals2 (sig_args sig) ->
+        Forall2 (val_inject j) vals1 vals2 ->
+        Mem.inject j m1 m2->*)
 
 (* LENB: we may want to add meminj_preserves_globals ge1 j as another asumption here,
       to get rid of meminj_preserved_globals_inject_incr below. But this would require spaeicaliing G1 to Genv.t....
@@ -528,81 +319,84 @@ Section Sim_INJ_SIMU_DIAGRAMS.
          mem_unchanged_on (loc_out_of_reach j m1) m2 m2' ->
          Val.has_type ret2 (proj_sig_res sig) ->
 
-        exists cd', exists st1', exists st2',
+      exists st1', exists st2', exists d',
           after_external Sem1 (Some ret1) st1 = Some st1' /\
           after_external Sem2 (Some ret2) st2 = Some st2' /\
-          match_state cd' j' st1' m1' st2' m2'. 
+          d' = st1' /\ match_states d' j' st1' m1' st2' m2'. 
+
+Section INJ_SIMULATION_STAR_WF.
+Variable order: C1 -> C1 -> Prop.
+Hypothesis order_wf: well_founded order.
+
+  Hypothesis inj_simulation:
+     forall c1 m1 c1' m1',  corestep Sem1 ge1 c1 m1 c1' m1' ->
+     forall j c2 m2, match_states c1 j c1 m1 c2 m2 ->
+      exists c2', exists m2', exists j', 
+                  inject_incr j j' /\
+                  inject_separated j j' m1 m2 /\
+                  match_states c1' j' c1' m1' c2' m2' /\
+                  (corestep_plus Sem2 ge2  c2 m2 c2' m2' \/ (corestep_star Sem2 ge2 c2 m2 c2' m2' /\ order c1' c1)).
+
+Lemma  inj_simulation_star_wf: Sim_inj.Forward_simulation_inject _ _ Sem1 Sem2 ge1 ge2 entry_points.
+Proof.
+  eapply Sim_inj.Build_Forward_simulation_inject with
+        (core_ord := order)
+        (match_state := fun d j c1 m1 c2 m2 => d = c1 /\ match_states d j c1 m1 c2 m2).
+   apply order_wf.
+   intros. destruct H0; subst.
+              destruct (inj_simulation _ _ _ _ H _ _ _ H1) as [c2' [m2' [j' [INC [SEP [MC' Step]]]]]].
+              exists c2'. exists m2'. exists st1'. exists j'.  split; eauto.
+   intros. destruct (match_initial_cores _ _ _ H _ _ _ _ _ _ H0 H1 H2 H3) as [c2' [MIC MC]].
+                 exists c1.  exists c2'. split; eauto.
+   intros. destruct H; subst. eapply inj_safely_halted; eauto.
+   intros.  destruct H; subst. eapply inj_at_external; eauto.
+   intros.  (*destruct H0; subst.*) clear inj_simulation .
+         specialize (inj_after_external _ _ _ _ _ _ _ _ _ _ _ _ _ _ H0 H1 H2 H3 H4 H5 H6 H7 H8 H9 H10 H11).
+          destruct inj_after_external as [c1' [c2' [d' [X1 [X2 [X3 X4]]]]]]. subst.
+           exists c1'. exists c1'. exists c2'. split; auto.
+Qed.
+End INJ_SIMULATION_STAR_WF.
 
 Section INJ_SIMULATION_STAR.
-  Variable measure: C1 -> nat. 
-  Definition inj_star_data : Type := (core_data * C1)%type.
-  Definition inj_star_ord:= lex_ord order (ltof _ measure).
- 
-  Definition inj_match_states_star (cd:inj_star_data) j (c1:  C1) m1 (c2: C2) m2 : Prop :=
-       match cd with (d,c) => match_state d j c1 m1 c2 m2 \/ (lt (measure c) (measure c1) /\ match_state d j c m1 c2 m2)
-       end.
-
-  Hypothesis inj_star_halted_Zero:  forall c1 v, safely_halted Sem1 ge1 c1 = Some v -> measure c1 = O.
-  Hypothesis inj_star_atExt_Zero:  forall c1 v, at_external Sem1 c1 = Some v -> measure c1 = O.
-
- Hypothesis inj_star_sim_diag:  forall c1 m1 c1' m1' (CS: corestep Sem1 ge1 c1 m1 c1' m1')
-                       dc c2 j m2 (MCS:inj_match_states_star dc j c1 m1 c2 m2),
-                      exists c2', exists m2', exists dc', exists j',
-          inject_incr j j' /\
-          inject_separated j j' m1 m2 /\
-          inj_match_states_star dc' j' c1' m1' c2' m2' /\
-          ((corestep_plus Sem2 ge2 c2 m2 c2' m2') \/
-            corestep_star Sem2 ge2 c2 m2 c2' m2' /\
-            inj_star_ord dc' dc).
+  Variable measure: C1 -> nat.
+  
+  Hypothesis inj_star_simulation:
+    forall c1 m1 c1' m1', corestep Sem1 ge1 c1 m1 c1' m1'  -> 
+    forall c2 m2 j, match_states c1 j c1 m1 c2 m2 ->
+      (exists c2', exists m2', exists j', 
+                  inject_incr j j' /\
+                  inject_separated j j' m1 m2 /\ 
+                  corestep_plus Sem2 ge2 c2 m2 c2' m2' /\ (*apparently not needed: Mem.inject j' m1' m2' /\ *) match_states c1' j' c1' m1' c2' m2')
+     \/ (measure c1' < measure c1 /\ (*apparently not needed: Mem.inject j m1' m2 /\ *) match_states c1' j c1' m1' c2 m2)%nat.
 
 Lemma  inj_simulation_star: Sim_inj.Forward_simulation_inject _ _ Sem1 Sem2 ge1 ge2 entry_points.
 Proof.
-  eapply Sim_inj.Build_Forward_simulation_inject with (core_ord:= inj_star_ord). (*(match_state:=inj_match_states_star).*)
-      eapply wf_lex_ord. apply order_wf.  apply (well_founded_ltof _ measure).
-   apply inj_star_sim_diag.
-   intros. clear  inj_safely_halted inj_at_external inj_after_external inj_star_sim_diag.
-          specialize (match_initial_cores _ _ _ H _ _ _ _ _ _ H0 H1 H2 H3).
-          destruct match_initial_cores as [d [c2 [Ini2 Mtch]]]; clear match_initial_cores.
-          exists (d,c1). exists c2. split; trivial.  left.  trivial.
-   intros. clear  inj_at_external inj_after_external inj_star_sim_diag match_initial_cores inj_star_sim_diag.
-        assert (X:= inj_star_halted_Zero _ _ H0).
-         destruct cd as [d c]. destruct H. eapply inj_safely_halted . apply H. apply H0.
-         destruct H. rewrite X in H. inv H.
-   intros. clear inj_star_sim_diag inj_safely_halted  inj_after_external match_initial_cores inj_star_halted_Zero.
-           assert (X:= inj_star_atExt_Zero _ _ H0).
-        destruct cd as [d c]. destruct H.
-          eapply inj_at_external ; eauto. 
-        destruct H. rewrite X in H. inv H.
-   intros. clear inj_star_sim_diag inj_safely_halted  match_initial_cores inj_star_halted_Zero inj_at_external.
-           destruct cd as [d c]. 
-           destruct H0. specialize (inj_after_external _ _ _ _ _ _ _ _ _ _ _ _ _ _ H H0 H1 H2 H3 H4 H5 H6 H7 H8 H9 H10 H11).
-                destruct inj_after_external  as [d' [c1' [c2' [AftExt1 [AftExt2 MC]]]]].
-                exists (d',c).  exists c1'. exists c2'. split; trivial. split; trivial. left. assumption.
-          destruct H0. rewrite (inj_star_atExt_Zero _ _ H1) in H0. inv H0.
+  eapply inj_simulation_star_wf.
+        apply  (well_founded_ltof _ measure).
+        intros. destruct (inj_star_simulation _ _ _ _ H _ _ _ H0).
+             destruct H1 as [c2' [m2' [j' [INC [ SEP [CSP MC']]]]]]. exists c2'. exists m2'. exists j'. split; trivial. split; trivial. split; trivial. left; trivial.
+             destruct H1 as [X1 X3]; subst. exists c2. exists m2. exists j.
+                   split. apply inject_incr_refl.
+                   split. apply inject_separated_same_meminj. 
+                   split; trivial. right. split; trivial.
+             eapply corestep_star_zero. 
 Qed.
 End INJ_SIMULATION_STAR.
 
 Section INJ_SIMULATION_PLUS.
- Hypothesis inj_plus_sim_diag:   forall c1 m1 c1' m1' (CS: corestep Sem1 ge1 c1 m1 c1' m1')
-                       dc c2 j m2 (MCS:inj_match_states_star (fun _ => O) dc j c1 m1 c2 m2),
-        exists c2', exists m2', exists dc', exists j',
-          inject_incr j j' /\
-          inject_separated j j' m1 m2 /\
-          inj_match_states_star (fun _ => O) dc' j' c1' m1' c2' m2' /\
-          corestep_plus Sem2 ge2 c2 m2 c2' m2'.
+  Variable measure: C1 -> nat. 
+  Hypothesis inj_plus_simulation:
+    forall c1 m1 c1' m1', corestep Sem1 ge1 c1 m1 c1' m1'  -> 
+    forall c2 m2 j, match_states c1 j c1 m1 c2 m2 ->
+            exists c2', exists m2',  exists j', 
+                  inject_incr j j' /\
+                  inject_separated j j' m1 m2 /\ corestep_plus Sem2 ge2 c2 m2 c2' m2' /\ match_states c1' j' c1' m1' c2' m2'.
 
 Lemma  inj_simulation_plus: Sim_inj.Forward_simulation_inject _ _ Sem1 Sem2 ge1 ge2 entry_points.
 Proof.
-  apply inj_simulation_star with (measure := fun _ => O).
-      intros. trivial.
-      intros. trivial.
-      intros.
-               clear inj_after_external inj_at_external inj_safely_halted match_initial_cores.
-               destruct (inj_plus_sim_diag _ _ _ _ CS _ _ _ _ MCS) as [c2' [m2' [dc' [j' [InjInc [InjSep [MCS' CSP]]]]]]].
-               exists c2'. exists m2'. exists dc'. exists j'.  split. assumption. split. assumption.  split. assumption. left. trivial.
+  apply inj_simulation_star with (measure:=measure).
+        intros. destruct (inj_plus_simulation _ _ _ _ H _ _ _ H0).
+             left. eexists; eauto.
 Qed.
-
 End INJ_SIMULATION_PLUS.
 End Sim_INJ_SIMU_DIAGRAMS.
-
-
